doc/coq/signature/ALinking.v
@@ -1,360 +1,164 @@
 From Signature Require Export Abstract.
-Require Export Coq.Logic.FunctionalExtensionality.
 
 Generalizable Variables T BT AT.
 
-Definition plugin_ctx_mem `{Eq T} (Cout : @dy_ctx T) (mem : T -> list expr_value) :=
-  fun t => map (plugin_ctx_v Cout) (mem t).
-
-Definition delete_ctx_mem `{Eq T} (Cout : @dy_ctx T) (mem : T -> list expr_value) :=
-  fun t => map (delete_ctx_v Cout) (mem t).
-
-Lemma delete_ctx_mem_eq :
-  forall `{Eq T} (Cout : @dy_ctx T) (mem : T -> list expr_value),
-         delete_ctx_mem Cout (plugin_ctx_mem Cout mem) = mem.
-Proof.
-  intros. apply functional_extensionality.
-  intros. unfold plugin_ctx_mem. unfold delete_ctx_mem.
-  remember (mem x) as l. clear Heql x mem. revert Cout.
-  induction l; try reflexivity. intros.
-  destruct a; simpl;
-  rewrite delete_eq;
-  rewrite IHl; reflexivity.
-Qed.
-
-Inductive link {BT AT} :=
-  | BF (t : BT)
-  | AF (t : AT)
-.
-
-Definition link_eqb `{Eq BT} `{Eq AT} (t t' : @link BT AT) :=
-  match t, t' with
-  | BF t, BF t' => eqb t t'
-  | AF t, AF t' => eqb t t'
-  | _, _ => false
-  end.
-
-Lemma link_eqb_eq `{Eq BT} `{Eq AT} :
-  forall (t t' : @link BT AT), link_eqb t t' = true <-> t = t'.
-Proof.
-  intros.
-  destruct t; destruct t'; simpl; split; intros EQ; 
-  try rewrite eqb_eq in *;
-  try inversion EQ;
-  subst; eauto.
-Qed.
-
-Lemma link_eqb_neq `{Eq BT} `{Eq AT} :
-  forall (t t' : @link BT AT), link_eqb t t' = false <-> t <> t'.
-Proof.
-  intros. split; intros NEQ.
-  - red. intros contra. rewrite <- link_eqb_eq in contra.
-    rewrite NEQ in contra. inversion contra.
-  - refl_bool. intros contra. rewrite link_eqb_eq in contra.
-    apply NEQ. eauto.
-Qed.
-
-#[export] Instance link_eq `{Eq BT} `{Eq AT} : Eq (@link BT AT) :=
-  {
-    eqb := link_eqb;
-    eqb_eq := link_eqb_eq;
-    eqb_neq := link_eqb_neq
-  }.
-
-Fixpoint filter_ctx_bf {BT AT} (C : @dy_ctx (@link BT AT)) :=
-  match C with
-  | [||] => [||]
-  | dy_binde x t C' =>
+Definition link_tick `{time BT} `{time AT} (Cout : dy_ctx BT) :=
+  fun C m t x v =>
     match t with
-    | BF t => dy_binde x t (filter_ctx_bf C')
-    | AF t => filter_ctx_bf C'
-    end
-  | dy_bindm M C' C'' => dy_bindm M (filter_ctx_bf C') (filter_ctx_bf C'')
-  end.
-
-Fixpoint filter_ctx_af {BT AT} (C : @dy_ctx (@link BT AT)) :=
-  match C with
-  | [||] => [||]
-  | dy_binde x t C' =>
-    match t with
-    | AF t => dy_binde x t (filter_ctx_af C')
-    | BF t => filter_ctx_af C'
-    end
-  | dy_bindm M C' C'' => dy_bindm M (filter_ctx_af C') (filter_ctx_af C'')
-  end.
-
-Definition filter_v_bf {BT AT} (v : @expr_value (@link BT AT)) :=
-  match v with
-  | Fun x e C => Fun x e (filter_ctx_bf C)
-  | Func M s e C => Func M s e (filter_ctx_bf C)
-  end.
-
-Definition filter_v_af {BT AT} (v : @expr_value (@link BT AT)) :=
-  match v with
-  | Fun x e C => Fun x e (filter_ctx_af C)
-  | Func M s e C => Func M s e (filter_ctx_af C)
-  end.
-
-Definition filter_mem_bf {BT AT} (mem : (@link BT AT) -> list (@expr_value (@link BT AT))) :=
-  fun t => map filter_v_bf (mem (BF t))
-.
-
-Definition filter_mem_af {BT AT} (mem : (@link BT AT) -> list (@expr_value (@link BT AT))) :=
-  fun t => map filter_v_af (mem (AF t))
-.
-
-Fixpoint lift_ctx_bf {BT AT} C : @dy_ctx (@link BT AT) :=
-  match C with
-  | [||] => [||]
-  | dy_binde x t C' => dy_binde x (BF t) (lift_ctx_bf C')
-  | dy_bindm M C' C'' => dy_bindm M (lift_ctx_bf C') (lift_ctx_bf C'')
-  end.
-
-Definition lift_v_bf {BT AT} v : @expr_value (@link BT AT) :=
-  match v with
-  | Fun x e C => Fun x e (lift_ctx_bf C)
-  | Func M s e C => Func M s e (lift_ctx_bf C)
-  end.
-
-Fixpoint lift_ctx_af {BT AT} C : @dy_ctx (@link BT AT) :=
-  match C with
-  | [||] => [||]
-  | dy_binde x t C' => dy_binde x (AF t) (lift_ctx_af C')
-  | dy_bindm M C' C'' => dy_bindm M (lift_ctx_af C') (lift_ctx_af C'')
-  end.
-
-Definition lift_v_af {BT AT} v : @expr_value (@link BT AT) :=
-  match v with
-  | Fun x e C => Fun x e (lift_ctx_af C)
-  | Func M s e C => Func M s e (lift_ctx_af C)
-  end.
-
-Definition link_tick `{Eq BT} `{time AT} (Cout : @dy_ctx BT) :=
-  fun C st x v =>
-    match st with
-    | ST mem t =>
-      match t with
-      | BF t => BF t
-      | AF t =>
-        let Cout := lift_ctx_bf Cout in
-        AF
-        (tick (filter_ctx_af (delete Cout C))
-                (ST (filter_mem_af (delete_ctx_mem Cout mem)) t)
-                x (filter_v_af (delete_ctx_v Cout v)))
-      end
+    | BF t => BF (tick (filter_ctx_bf C) (filter_mem_bf m) t x (filter_v_bf v))
+    | AF t =>
+      let Cout := lift_ctx_bf Cout in
+      AF (tick (filter_ctx_af (delete eqb Cout C))
+            (filter_mem_af (delete_ctx_mem eqb Cout m)) t
+            x (filter_v_af (delete_v eqb Cout v)))
     end.
 
-#[export] Instance link_time `{Eq BT} `{time AT} (Cout : @dy_ctx BT) : (@time (@link BT AT) (@link_eq BT _ AT _)) :=
+Lemma link_tick_ext `{time BT} `{time AT} (Cout : dy_ctx BT) :
+  forall C m m' t x v (SAME : asame m m'),
+  link_tick Cout C m t x v = link_tick Cout C m' t x v.
+Proof.
+  intros. destruct t; simpl;
+  match goal with
+  | |- BF ?a = BF ?b =>
+    assert (a = b) as RR;
+    first [rewrite RR; reflexivity | apply tick_ext]
+  | |- AF ?a = AF ?b =>
+    assert (a = b) as RR;
+    first [rewrite RR; reflexivity | apply tick_ext]
+  end; unfold asame in *; ii;
+  match goal with
+  | |- In ?v (aread (filter_mem_bf _) ?t) <-> _ =>
+    specialize (SAME (BF t));
+    repeat rewrite aread_filter_bf;
+    split; i; des; clarify; eexists; split;
+    try reflexivity; rewrite SAME in *; assumption
+  | |- In ?v (aread (filter_mem_af _) ?t) <-> _ =>
+    specialize (SAME (AF t));
+    repeat rewrite aread_filter_af;
+    split; i; des; clarify; eexists; split;
+    try reflexivity; rewrite aread_delete in *;
+    des; clarify; eexists; split;
+    try reflexivity; rewrite SAME in *; assumption
+  end.
+Qed.
+
+#[export] Instance link_time `{time BT} `{time AT} (Cout : dy_ctx BT) : (@time (link BT AT) (@link_eq BT _ AT _ )) :=
   {
-    tick := link_tick Cout
+    tick := link_tick Cout;
+    tick_ext := link_tick_ext Cout;
   }.
 
-Definition link_mem `{Eq BT} `{Eq AT}
-  (bmem : BT -> list (@expr_value BT)) (Cout : @dy_ctx BT)
-  (amem : AT -> list (@expr_value AT)) : (@link BT AT) -> list (@expr_value (@link BT AT)):=
-  fun t =>
-    match t with
-    | BF t => map lift_v_bf (bmem t)
-    | AF t => map (plugin_ctx_v (lift_ctx_bf Cout)) (map (lift_v_af) (amem t))
-    end.
-
-Lemma filter_lift_eq_af {BT AT} :
-  forall (C : @dy_ctx AT),
-    filter_ctx_af (@lift_ctx_af BT AT C) = C.
-Proof.
-  induction C; simpl; try rewrite IHC; eauto.
-  rewrite IHC2. rewrite IHC1. eauto.
-Qed.
-
-Lemma filter_lift_eq_bf {BT AT} :
-  forall (C : @dy_ctx BT),
-    filter_ctx_bf (@lift_ctx_bf BT AT C) = C.
-Proof.
-  induction C; simpl; try rewrite IHC; eauto.
-  rewrite IHC2. rewrite IHC1. eauto.
-Qed.
-
-Lemma filter_delete_eq `{Eq BT} `{time AT} (Cout : @dy_ctx BT):
-  forall bmem amem,
-  filter_mem_af
-    (delete_ctx_mem (lift_ctx_bf Cout)
-    (link_mem bmem Cout amem)) = amem.
-Proof.
-  intros. apply functional_extensionality.
-  intros. unfold filter_mem_af.
-  unfold delete_ctx_mem. simpl.
-  remember (lift_ctx_bf Cout) as vout eqn:E. clear E.
-  remember (amem x) as l eqn:E. clear E.
-  induction l; simpl; eauto.
-  rewrite IHl; destruct a; simpl;
-  rewrite delete_eq; rewrite filter_lift_eq_af; reflexivity.
-Qed.
-
-Lemma link_tick_eq `{Eq BT} `{time AT} (Cout : @dy_ctx BT) :
+Lemma link_tick_eq `{time BT} `{time AT} (Cout : @dy_ctx BT) :
   forall bmem C amem t x v,
-    link_tick Cout ((lift_ctx_bf Cout)[|(lift_ctx_af C)|])
-                (ST (link_mem bmem Cout amem) (AF t)) x 
-                (plugin_ctx_v (lift_ctx_bf Cout) (lift_v_af v)) =
-    AF (tick C (ST amem t) x v).
+    link_tick Cout ((lift_ctx_af C)[|(lift_ctx_bf Cout)|])
+                (link_mem bmem Cout amem) (AF t) x 
+                (inject_v (lift_ctx_bf Cout) (lift_v_af v)) =
+    AF (tick C amem t x v).
 Proof.
-  intros. destruct v; unfold plugin_ctx_v; simpl;
-  rewrite delete_eq;
-  rewrite delete_eq;
-  rewrite filter_delete_eq;
-  rewrite filter_lift_eq_af; rewrite filter_lift_eq_af;
+  intros. destruct v; unfold inject_v; simpl;
+  repeat rewrite delete_inject_eq;
+  repeat rewrite filter_delete_eq;
+  repeat rewrite filter_lift_eq_af; 
+  repeat rewrite filter_lift_eq_af;
+  ii;
+  repeat rewrite link_eqb_eq;
   reflexivity.
 Qed.
 
-Lemma link_update_m_eq `{Eq BT} `{time AT} (Cout : @dy_ctx BT):
-  forall bmem amem t v,
-  (AF t !#-> plugin_ctx_v (lift_ctx_bf Cout) (lift_v_af v);
-    (link_mem bmem Cout amem)) =
-    link_mem bmem Cout (t !#-> v; amem).
+Lemma lift_inject {BT AT} :
+  forall (C1 C2 : dy_ctx AT),
+    @lift_ctx_af BT _ (C1 [|C2|]) = (lift_ctx_af C1 [|lift_ctx_af C2|]).
 Proof.
-  intros. apply functional_extensionality.
-  intros. unfold update_m. destruct v; simpl;
-  destruct x; simpl; eauto;
-  destruct (eqb t0 t); eauto.
+  induction C1; ii; ss; rw; eauto.
 Qed.
 
-Lemma lift_addr_x {BT AT} :
-  forall (C : @dy_ctx AT) x,
-    addr_x (lift_ctx_af C : @dy_ctx (@link BT AT)) x =
-      match addr_x C x with
-      | Some addr => Some (AF addr)
-      | None => None
-      end.
+Lemma lift_project {BT AT} :
+  forall s (C : dy_ctx AT) Cs (PROJ : project C s = Some Cs),
+    project (@lift_ctx_af BT _ C) s = Some (@lift_ctx_af BT _ Cs).
 Proof.
-  induction C; simpl; eauto;
-  intros;
-  destruct (eq_eid x0 x); rewrite IHC;
-  destruct (addr_x C x0); eauto.
+  induction s; ii; ss; clarify;
+  repeat des_hyp;
+  clarify.
+  erewrite IHs; eauto.
+  rewrite lift_addr_x. rw. eauto.
+  rewrite lift_ctx_M. rw.
+  erewrite IHs1; eauto.
+  erewrite IHs2; eauto. s. eauto.
 Qed.
 
-Lemma lift_ctx_M {BT AT} :
-  forall (C : @dy_ctx AT) M,
-    ctx_M (lift_ctx_af C : @dy_ctx (@link BT AT)) M =
-      match ctx_M C M with
-      | Some CM => Some (lift_ctx_af CM)
-      | None => None
-      end.
+Theorem link_step_eq `{time BT} `{time AT} (Cout : dy_ctx BT) :
+  forall bmem e C m t cf'
+    (EVAL : {|(Cf e C m t) ~#> cf'|}),
+    (@step (link BT AT) _ (link_time Cout)
+      (inject_cf Cout bmem (Cf e C m t))
+      (inject_cf Cout bmem cf')).
 Proof.
-  induction C; simpl; eauto;
-  intros.
-  destruct (eq_mid M0 M); rewrite IHC2;
-  destruct (ctx_M C2 M0); eauto.
-Qed.
-
-Lemma lift_plugin_af {BT AT} :
-  forall (C C' : @dy_ctx AT),
-    @lift_ctx_af BT AT (C[|C'|]) = (lift_ctx_af C [|lift_ctx_af C'|]).
-Proof.
-  induction C; simpl; intros; try rewrite IHC; eauto.
-  rewrite IHC2. eauto.
-Qed.
-
-Lemma project_lift {BT AT} :
-  forall (s : st_ctx) (C CM : @dy_ctx AT) (PROJ : Some CM = project C s),
-    Some (lift_ctx_af CM : @dy_ctx (@link BT AT)) = project (lift_ctx_af C) s.
-Proof.
-  intros s. induction s; intros; inversion PROJ; subst; eauto.
-  - simpl. destruct (addr_x C x) eqn:ADDR; inversion H0.
-    pose proof (@lift_addr_x BT AT C x) as RR. rewrite ADDR in RR.
-    rewrite RR.
-    destruct (project C s) eqn:PROJs; inversion H0.
-    erewrite <- IHs; eauto. simpl. eauto.
-  - simpl. destruct (ctx_M C M) eqn:CTX; inversion H0.
-    pose proof (@lift_ctx_M BT AT C M) as RR. rewrite CTX in RR.
-    rewrite RR.
-    destruct (project d s1) eqn:PROJs1; inversion H0.
-    destruct (project C s2) eqn:PROJs2; inversion H2.
-    erewrite <- IHs1; eauto.
-    erewrite <- IHs2; eauto. simpl. eauto.
-Qed.
-
-Lemma link_eval_eq `{Eq BT} `{time AT} (Cout : @dy_ctx BT) :
-  forall bmem C st e v st'
-         (EVAL : @EvalR AT _ _ C st e v st'),
-    let inject_C := (lift_ctx_bf Cout) [|(lift_ctx_af C)|] in
-    let inject_v :=
-      match v with
-      | EVal ev => EVal (plugin_ctx_v (lift_ctx_bf Cout) (lift_v_af ev))
-      | MVal C_v => MVal ((lift_ctx_bf Cout)[|(lift_ctx_af C_v)|])
-      end in
-    let inject_st :=
-      match st with
-      | ST amem t => ST (link_mem bmem Cout amem) (AF t)
-      end in
-    let inject_st' :=
-      match st' with
-      | ST amem' t' => ST (link_mem bmem Cout amem') (AF t')
-      end in
-    @EvalR (@link BT AT) _ (link_time Cout)
-      inject_C inject_st e inject_v inject_st'.
-Proof.
-  intros. induction EVAL;
-  try destruct st; try destruct st'; try destruct st'';
-  try (destruct inject_v eqn:INJv; inversion INJv; subst);
-  try (destruct inject_st eqn:INJst; inversion INJst; subst);
-  try (destruct inject_st' eqn:INJst'; inversion INJst'; subst); eauto.
-  - inversion STATE; subst.
-    eapply Eval_e_var; eauto.
-    pose proof (plugin_ctx_addr_x x (lift_ctx_bf Cout) (lift_ctx_af C)) as RR.
-    rewrite lift_addr_x in RR.
-    rewrite <- ADDR in RR. symmetry. apply RR.
-    unfold link_mem. 
-    remember (mem0 addr) as l.
-    clear Heql inject_C C mem0 x addr t0 inject_st' INJst' STATE inject_st INJst ADDR inject_v INJv.
-    induction l; simpl; intros; eauto.
-    destruct ACCESS as [L | R].
-    left. rewrite L. eauto.
-    right. apply IHl. eauto.
-  - destruct st_v.
-    eapply Eval_e_app_fn; try apply IHEVAL1; try apply IHEVAL2.
-    pose proof (link_tick_eq Cout bmem C mem t x arg) as RR.
-    simpl in *. subst inject_C.
-    rewrite RR. clear RR.
-    pose proof (link_update_m_eq Cout bmem mem t arg) as RR. simpl in RR.
-    rewrite RR. clear RR.
-    rewrite <- dy_plugin_assoc. rewrite lift_plugin_af in IHEVAL3. eauto.
-  - destruct st_v. destruct st_arg.
-    eapply Eval_e_app_ft with (CM := lift_ctx_af CM);
-    try apply IHEVAL1; try apply IHEVAL2;
-    try (rewrite <- dy_plugin_assoc; rewrite lift_plugin_af in IHEVAL3; eauto).
-    pose proof (@project_lift BT AT) as RR.
-    specialize (RR s_lam arg CM PROJ).
-    rewrite RR. erewrite plugin_project_eq; eauto. 
-  - pose proof (plugin_ctx_ctx_M M (lift_ctx_bf Cout) (lift_ctx_af C)) as RR.
-    rewrite lift_ctx_M in RR.
-    rewrite <- ACCESS in RR. subst inject_C.
-    rewrite lift_plugin_af. rewrite dy_plugin_assoc.
-    eapply Eval_m_var; eauto.
-  - destruct st_v.
-    pose proof (@project_lift BT AT s v proj_v PROJv) as HINT.
-    assert ((lift_ctx_bf Cout [|lift_ctx_af (C [|proj_v|])|]) = 
-            ((lift_ctx_bf Cout [|lift_ctx_af C|]) [|lift_ctx_af proj_v|])) as RR.
-    { rewrite lift_plugin_af. rewrite dy_plugin_assoc. eauto. }
-    rewrite RR. clear RR.
-    eapply Eval_m_app_fn with (v := lift_ctx_bf Cout [|lift_ctx_af v|]);
-    try apply IHEVAL1; try apply IHEVAL2; eauto.
-    pose proof (link_tick_eq Cout bmem C mem t x arg) as RR.
-    simpl in *. subst inject_C.
-    rewrite RR. clear RR.
-    pose proof (link_update_m_eq Cout bmem mem t arg) as RR. simpl in RR.
-    rewrite RR. clear RR.
-    rewrite <- dy_plugin_assoc. rewrite lift_plugin_af in IHEVAL3. eauto.
-    erewrite plugin_project_eq; eauto.
-  - destruct st_v. destruct st_arg.
-    pose proof (@project_lift BT AT s_lam arg CM PROJ) as HINT.
-    pose proof (@project_lift BT AT s v proj_v PROJv) as HINTv.
-    assert ((lift_ctx_bf Cout [|lift_ctx_af (C [|proj_v|])|]) = 
-            ((lift_ctx_bf Cout [|lift_ctx_af C|]) [|lift_ctx_af proj_v|])) as RR.
-    { rewrite lift_plugin_af. rewrite dy_plugin_assoc. eauto. }
-    rewrite RR. clear RR.
-    eapply Eval_m_app_ft with 
-      (v := lift_ctx_bf Cout [|lift_ctx_af v|])
-      (CM := lift_ctx_af CM);
-    try apply IHEVAL1; try apply IHEVAL2; eauto;
-    try (erewrite plugin_project_eq; eauto).
-    rewrite <- dy_plugin_assoc. rewrite lift_plugin_af in IHEVAL3. eauto.
+  intros. remember (Cf e C m t) as cf.
+  ginduction EVAL; ii; ss; repeat des_goal; repeat des_hyp; clarify;
+  repeat rewrite lift_inject in *;
+  repeat rewrite inject_assoc in *;
+  repeat match goal with
+  | PROJ : project ?C _ = Some _ |- _ =>
+    lazymatch type of C with
+    | dy_ctx (link _ _) => fail
+    | _ =>
+      eapply (@lift_project BT) in PROJ;
+      eapply (plugin_project_eq (lift_ctx_bf Cout)) in PROJ
+    end
+  end;
+  match goal with
+  | ADDR : addr_x ?Cin ?x = Some ?addr,
+    ACCESS : In (Fun ?x_lam ?e ?C) (aread ?m ?addr)
+    |- context[ (lift_ctx_af ?Cin) [|lift_ctx_bf ?Cout|] ] =>
+    let RR := fresh "RR" in
+    pose proof (inject_addr_x x (lift_ctx_bf Cout) (lift_ctx_af Cin));
+    pose proof (@lift_addr_x BT AT Cin x) as RR;
+    rewrite ADDR in *; rewrite RR in *;
+    assert (In (Fun x_lam e (lift_ctx_af C [|lift_ctx_bf Cout|])) 
+      (aread (link_mem bmem Cout m) (AF addr)));
+    first[
+      unfold link_mem; rewrite aread_in; rewrite aread_in in ACCESS;
+      rewrite in_app_iff; left;
+      induction m; ss; des; des_goal; clarify; ss; eauto
+      | eauto]
+  | ADDR : addr_x ?Cin ?x = Some ?addr,
+    ACCESS : In (Func ?M ?s ?e ?C) (aread ?m ?addr)
+    |- context[ (lift_ctx_af ?Cin) [|lift_ctx_bf ?Cout|] ] =>
+    let RR := fresh "RR" in
+    pose proof (inject_addr_x x (lift_ctx_bf Cout) (lift_ctx_af Cin));
+    pose proof (@lift_addr_x BT AT Cin x) as RR;
+    rewrite ADDR in *; rewrite RR in *;
+    assert (In (Func M s e (lift_ctx_af C [|lift_ctx_bf Cout|])) 
+      (aread (link_mem bmem Cout m) (AF addr)));
+    first[
+      unfold link_mem; rewrite aread_in; rewrite aread_in in ACCESS;
+      rewrite in_app_iff; left;
+      induction m; ss; des; des_goal; clarify; ss; eauto
+      | eauto]
+  | ACCESS: ctx_M ?Cin ?M = _
+    |- context [lift_ctx_af ?Cin [|lift_ctx_bf ?Cout|] ] =>
+    let RR := fresh "RR" in
+    pose proof (@lift_ctx_M BT AT Cin M) as RR;
+    pose proof (inject_ctx_M M (lift_ctx_bf Cout) (lift_ctx_af Cin));
+    rewrite ACCESS in *;
+    rewrite RR in *; eauto
+  | _ => solve [exploit IHEVAL; eauto]
+  | _ =>
+    let RR := fresh "RR" in
+    let RRR := fresh "RRR" in
+    try (exploit IHEVAL1; eauto; instantiate (1 := Cout); instantiate (1 := bmem));
+    try (exploit IHEVAL2; eauto; instantiate (1 := Cout); instantiate (1 := bmem));
+    try (exploit IHEVAL3; eauto; instantiate (1 := Cout); instantiate (1 := bmem));
+    ii;
+    pose proof (@link_tick_eq BT _ _ AT _ _ Cout bmem) as RR;
+    pose proof (@link_update_m_eq BT _ AT _ Cout bmem) as RRR;
+    try rewrite <- RRR in *;
+    try rewrite <- RR in *;
+    pose proof (@FnEAppBody (link BT AT) _ (link_time Cout));
+    pose proof (@FnEApp (link BT AT) _ (link_time Cout));
+    pose proof (@FnMAppBody (link BT AT) _ (link_time Cout));
+    pose proof (@FnMApp (link BT AT) _ (link_time Cout));
+    simpl tick in *;
+    eauto
+  end.
 Qed.
