doc/coq/signature/Syntax.v
@@ -1,107 +1,135 @@
-From Coq Require Export Bool.Bool.
-From Coq Require Export Init.Nat.
-From Coq Require Export Arith.Arith.
-From Coq Require Export Arith.EqNat.
-From Coq Require Export Lia.
-From Coq Require Export Lists.List.
-From Coq Require Export Strings.String.
+From Basics Require Export Basics.
 
-Notation "x :: y" := (cons x y)
-                     (at level 60, right associativity).
-Notation "[ ]" := nil.
-Notation "[ x ; .. ; y ]" := (cons x .. (cons y []) ..).
-Notation "x ++ y" := (app x y)
-                     (at level 60, right associativity).
+(** Syntax of our language *)
+Definition ID := String.string.
 
-Inductive expr_id :=
-  | eid (x : nat)
-.
+Definition eqb_ID := String.eqb.
 
-Inductive mod_id :=
-  | mid (M : nat)
-.
+Definition eqb_ID_eq := String.eqb_eq.
 
-Definition eq_eid id1 id2 :=
-  match id1, id2 with
-  | eid x1, eid x2 => x1 =? x2
-  end.
+#[export] Instance EqID : Eq ID := { eqb:= eqb_ID; eqb_eq := eqb_ID_eq; }.
 
-Definition eq_mid id1 id2 :=
-  match id1, id2 with
-  | mid M1, mid M2 => M1 =? M2
-  end.
+Definition eqb_ID_neq := String.eqb_neq.
 
-Lemma eq_eid_eq : forall x x',
-  eq_eid x x' = true <-> x = x'.
-Proof.
-  intros. destruct x. destruct x'.
-  simpl. split; intros. 
-  rewrite Nat.eqb_eq in H.
-  rewrite H. eauto.
-  inversion H; subst. rewrite Nat.eqb_eq. eauto.
-Qed.
-
-Lemma eq_eid_neq : forall x x',
-  eq_eid x x' = false <-> x <> x'.
-Proof.
-  intros. destruct x. destruct x'.
-  simpl. split; intros.
-  unfold not. intros.
-  rewrite Nat.eqb_neq in H. apply H. inversion H0. eauto.
-  rewrite Nat.eqb_neq. unfold not. intros. apply H. subst; eauto.
-Qed.
-
-Lemma eq_mid_eq : forall M M',
-  eq_mid M M' = true <-> M = M'.
-Proof.
-  intros. destruct M. destruct M'.
-  simpl. split; intros. 
-  rewrite Nat.eqb_eq in H.
-  rewrite H. eauto.
-  inversion H; subst. rewrite Nat.eqb_eq. eauto.
-Qed.
-
-Lemma eq_mid_neq : forall M M',
-  eq_eid M M' = false <-> M <> M'.
-Proof.
-  intros. destruct M. destruct M'.
-  simpl. split; intros.
-  unfold not. intros.
-  rewrite Nat.eqb_neq in H. apply H. inversion H0. eauto.
-  rewrite Nat.eqb_neq. unfold not. intros. apply H. subst; eauto.
-Qed.
+Lemma ID_refl : forall x, eqb_ID x x = true.
+Proof. intros; apply eqb_ID_eq; eauto. Qed.
 
 Inductive st_ctx :=
   | st_hole
-  | st_binde (x : expr_id) (C : st_ctx)
-  | st_bindm (M : mod_id) (CM : st_ctx) (C : st_ctx)
+  | st_binde (x : ID) (C : st_ctx)
+  | st_bindm (M : ID) (CM : st_ctx) (C : st_ctx)
 .
 
+Notation "'[[|' '|]]'" := (st_hole) (at level 99).
+
 Inductive tm :=
-  | e_var (x : expr_id)
-  | e_lam (x : expr_id) (e : tm)
+  | e_var (x : ID)
+  | e_lam (x : ID) (e : tm)
   | e_app (e1 : tm) (e2 : tm)
   | e_link (m : tm) (e : tm)
   | m_empty
-  | m_var (M : mod_id)
-  | m_lam (M : mod_id) (s : st_ctx) (e : tm)
+  | m_var (M : ID)
+  | m_lam (M : ID) (s : st_ctx) (e : tm)
   | m_app (e1 : tm) (e2 : tm) (s : st_ctx)
 .
 
+Fixpoint eqb_st s s' :=
+  match s, s' with
+  | ([[||]]), ([[||]]) => true
+  | st_binde x s, st_binde x' s' =>
+    eqb_ID x x' && eqb_st s s'
+  | st_bindm M sM s, st_bindm M' sM' s' =>
+    eqb_ID M M' && eqb_st sM sM' && eqb_st s s'
+  | _, _ => false
+  end.
+
+Lemma eqb_st_eq : forall s s', eqb_st s s' = true <-> s = s'.
+Proof.
+  induction s; ii; ss;
+  repeat des_goal; repeat des_hyp; ss;
+  try rewrite eqb_ID_eq in *;
+  try rewrite eqb_ID_neq in *;
+  split; ii; clarify;
+  try rewrite IHs in *;
+  try rewrite IHs1 in *;
+  try rewrite IHs2 in *;
+  clarify.
+  rrw. rw. eauto.
+Qed.
+
+#[export] Instance Eqst : Eq st_ctx := { eqb:= eqb_st; eqb_eq := eqb_st_eq; }.
+
+Ltac solve_eqb eqb_mine :=
+  assert (eqb_mine = eqb); eauto; rw.
+
+Lemma eqb_st_neq : forall s s', eqb_st s s' = false <-> s <> s'.
+Proof. solve_eqb eqb_st. exact eqb_neq. Qed.
+
+Lemma st_refl : forall s, eqb_st s s = true.
+Proof. solve_eqb eqb_st. exact t_refl. Qed.
+
+Fixpoint eqb_tm e e' :=
+  match e, e' with
+  | e_var x, e_var x' => eqb_ID x x'
+  | e_lam x e, e_lam x' e' => eqb_ID x x' && eqb_tm e e'
+  | e_app e1 e2, e_app e1' e2' => eqb_tm e1 e1' && eqb_tm e2 e2'
+  | e_link m e, e_link m' e' => eqb_tm m m' && eqb_tm e e'
+  | m_empty, m_empty => true
+  | m_var M, m_var M' => eqb_ID M M'
+  | m_lam M s e, m_lam M' s' e' =>
+    eqb_ID M M' && eqb_st s s' && eqb_tm e e'
+  | m_app e1 e2 s, m_app e1' e2' s' =>
+    eqb_tm e1 e1' && eqb_tm e2 e2' && eqb_st s s'
+  | _, _ => false
+  end.
+
+Lemma eqb_tm_eq : forall e e', eqb_tm e e' = true <-> e = e'.
+Proof.
+  induction e; intros; split; intros EQ; simpl in *;
+  destruct e'; try (inversion EQ; fail);
+  repeat des_hyp;
+  repeat match goal with
+  | [H : eqb_ID _ _ = true |- _] =>
+    rewrite eqb_ID_eq in H
+  | [H : eqb_st _ _ = true |- _] =>
+    rewrite eqb_st_eq in H
+  | [H : eqb_tm _ _ = true |- _] =>
+    repeat match goal with
+    | [RR : context [eqb_tm _ _ = true <-> _] |- _] =>
+      rewrite RR in H
+    end
+  | _ => idtac
+  end; subst; try reflexivity;
+  inversion EQ; subst;
+  try rewrite ID_refl; 
+  try rewrite st_refl; simpl; try reflexivity;
+  repeat match goal with
+  | [H : context [eqb_tm ?e _ = _] |- _] =>
+    match goal with
+    | [_ : eqb_tm e e = true |- _] => fail
+    | _ =>
+      let RR := fresh "RR" in
+      assert (eqb_tm e e = true) as RR;
+      try apply H; eauto; rewrite RR
+    end
+  | _ => fail
+  end.
+Qed.
+
+#[export] Instance Eqtm : Eq tm := { eqb := eqb_tm; eqb_eq := eqb_tm_eq; }.
+
+(** Statics *)
 Inductive value : tm -> Prop :=
   | v_fn x e : value (e_lam x e)
   | v_ft M s e : value (m_lam M s e)
 .
 
-Fixpoint st_ctx_M (C : st_ctx) (M : mod_id) :=
+Fixpoint st_ctx_M (C : st_ctx) (M : ID) :=
   match C with
-  | st_hole => None
+  | [[||]] => None
   | st_binde _ C' => st_ctx_M C' M
   | st_bindm M' CM' C' =>
-    match st_ctx_M C' M with
-    | Some CM => Some CM
-    | None => if eq_mid M M' then Some CM' else None
-    end
+    if eqb_ID M M' then Some CM' else st_ctx_M C' M
   end.
 
 Fixpoint st_plugin (Cout : st_ctx) (Cin : st_ctx) :=
@@ -111,26 +139,22 @@ Fixpoint st_plugin (Cout : st_ctx) (Cin : st_ctx) :=
   | st_bindm M' CM' C' => st_bindm M' CM' (st_plugin C' Cin)
   end.
 
-Lemma st_plugin_assoc : forall C1 C2 C3,
-  st_plugin (st_plugin C1 C2) C3 =
-  st_plugin C1 (st_plugin C2 C3). 
-Proof.
-  induction C1; eauto; 
-  intros; simpl; try rewrite IHC1; eauto.
-  rewrite IHC1_2. eauto.
-Qed.
-
 Notation "Cout '[[|' Cin '|]]'" := (st_plugin Cout Cin)
-                              (at level 100, Cin at next level, right associativity).
+  (at level 100, Cin at next level, right associativity).
 
-Notation "'[[||]]'" := (st_hole) (at level 100).
+Lemma st_plugin_assoc : forall C1 C2 C3,
+  C1 [[| C2 |]] [[| C3 |]] =
+    (C1 [[| C2 [[| C3 |]] |]]).
+Proof.
+  induction C1; eauto; ii; ss; repeat rw; eauto.
+Qed.
 
 (* collect all static contexts reachable from the current configuration *)
 Fixpoint collect_ctx C e :=
   match e with
   | e_var x => (None, [C])
   | e_lam x e' => 
-    let ctx_body := snd (collect_ctx (C [[|st_binde x ([[||]])|]]) e') in
+    let ctx_body := snd (collect_ctx (st_binde x C) e') in
     (None, C :: ctx_body)
   | e_app e1 e2 =>
     let ctxs1 := snd (collect_ctx C e1) in
@@ -146,296 +170,1228 @@ Fixpoint collect_ctx C e :=
   | m_empty => (Some C, [C])
   | m_var M =>
     match st_ctx_M C M with
-    | Some C_M => (Some (C[[|C_M|]]), [C])
+    | Some C_M => (Some (C_M[[|C|]]), C_M[[|C|]] :: [C])
     | None => (None, [C])
     end
   | m_lam M s e =>
-    let ctx_body := snd (collect_ctx (C [[|st_bindm M s ([[||]])|]]) e) in
+    let ctx_body := snd (collect_ctx (st_bindm M s C) e) in
     (None, C :: ctx_body)
   | m_app e1 e2 s =>
     let ctxs1 := snd (collect_ctx C e1) in
     let ctxs2 := snd (collect_ctx C e2) in
-    (Some (st_plugin C s), ctxs1 ++ ctxs2)
+    (Some (s[[|C|]]), s[[|C|]] :: ctxs1 ++ ctxs2)
   end.
+
+Lemma collect_ctx_refl : forall e C, In C (snd (collect_ctx C e)).
+Proof.
+  induction e; intros; simpl; eauto;
+  repeat des_goal;
+  try rewrite in_app_iff; first [left; eauto; fail | right; eauto; fail | eauto];
+  repeat match goal with
+  | [H : forall _ : st_ctx, In _ (snd (collect_ctx _ ?e)) |- _] =>
+    match goal with
+    | [RR : collect_ctx ?C e = _ |- _] =>
+      specialize (H C); rewrite RR in H
+    end
+  end; simpl in *; eauto.
+Qed.
 
 Lemma st_ctx_M_plugin :
   forall Cout Cin M,
-    st_ctx_M (st_plugin Cout Cin) M =
-      match st_ctx_M Cin M with
+    st_ctx_M (Cout[[|Cin|]]) M =
+      match st_ctx_M Cout M with
       | Some CM => Some CM
       | None =>
-        match st_ctx_M Cout M with
+        match st_ctx_M Cin M with
         | Some CM => Some CM
         | None => None
         end
       end.
 Proof.
-  induction Cout; intros; simpl; eauto.
-  - destruct (st_ctx_M Cin M); eauto.
-  - specialize (IHCout2 Cin M0). 
-    destruct (st_ctx_M Cin M0). 
-    rewrite IHCout2. eauto. 
-    rewrite IHCout2.
-    destruct (st_ctx_M Cout2 M0). eauto.
-    assert (RR : forall Cout0 Cin0, 
-    st_ctx_M (st_plugin Cout0 Cin0) M0 = None -> st_ctx_M Cin0 M0 = None).
-    { induction Cout0; intros; simpl; eauto. 
-      simpl in H. apply IHCout0_2.
-      destruct (st_ctx_M (st_plugin Cout0_2 Cin0) M0).
-      inversion H. eauto. }
-    specialize (IHCout1 Cin M0).
-    rewrite (RR Cout2 Cin IHCout2) in IHCout1.
-    destruct (eq_mid M0 M).
-    eauto. eauto.
+  induction Cout; ii; ss; des_goal; eauto.
 Qed.
 
-Lemma collect_ctx_refl : forall e C, In C (snd (collect_ctx C e)).
-Proof.
-  induction e; intros; simpl; eauto.
-  - apply in_app_iff. left. eauto.
-  - remember (collect_ctx C e1) as ol. destruct ol as [o l].
-    specialize (IHe1 C). rewrite <- Heqol in IHe1.
-    destruct o; eauto. simpl in *.
-    destruct (collect_ctx C e2); simpl in *.
-    destruct (collect_ctx s e2); simpl in *. 
-    apply in_app_iff. left. eauto.
-  - destruct (st_ctx_M C M); simpl; left; eauto.
-  - apply in_app_iff. eauto.
-Qed.
-
-(* dynamic context *)
-Inductive dy_ctx {time : Type} :=
+(** Dynamics *)
+Inductive dy_ctx T :=
   | dy_hole
-  | dy_binde (x: expr_id) (tx : time) (C : dy_ctx)
-  | dy_bindm (M : mod_id) (CM : dy_ctx) (C : dy_ctx)
+  | dy_binde (x : ID) (tx : T) (C : dy_ctx T)
+  | dy_bindm (M : ID) (CM : dy_ctx T) (C : dy_ctx T)
 .
 
-Fixpoint dy_plugin {time : Type} (Cout : @dy_ctx time) (Cin : @dy_ctx time) :=
-  match Cout with
-  | dy_hole => Cin
-  | dy_binde x tx C' => dy_binde x tx (dy_plugin C' Cin)
-  | dy_bindm M CM C' => dy_bindm M CM (dy_plugin C' Cin)
+Arguments dy_hole {T}.
+Arguments dy_binde {T}.
+Arguments dy_bindm {T}.
+
+Notation "'[|' '|]'" := (dy_hole) (at level 99).
+
+(* ctx inject *)
+Fixpoint inject {T} (C' C : dy_ctx T) :=
+  match C with
+  | [||] => C'
+  | dy_binde x tx C =>
+    dy_binde x tx (inject C' C)
+  | dy_bindm M CM C =>
+    dy_bindm M CM (inject C' C)
   end.
 
-Fixpoint addr_x {time : Type} (C : @dy_ctx time) (x : expr_id) :=
+Notation "C1 '[|' C2 '|]'" := (inject C2 C1)
+  (at level 100, C2 at next level, right associativity).
+
+Lemma inject_assoc {T} : forall (c1 c2 c3 : dy_ctx T),
+  c1 [| c2 |] [| c3 |] = (c1 [|c2 [|c3|]|]).
+Proof.
+  induction c1; ii; ss; rw; eauto.
+Qed.
+
+(* Auxiliary operators *)
+Fixpoint addr_x {T} (C : dy_ctx T) (x : ID) :=
   match C with
-  | dy_hole => None
+  | [||] => None
   | dy_binde x' tx' C' =>
-    match addr_x C' x with
-    | None => if eq_eid x x' then (Some tx') else None
-    | addr => addr
-    end
+    if eqb_ID x x' then (Some tx') else addr_x C' x
   | dy_bindm _ _ C' => addr_x C' x
   end.
 
-Fixpoint ctx_M {time : Type} (C : @dy_ctx time) (M : mod_id) :=
+Fixpoint ctx_M {T} (C : dy_ctx T) (M : ID) :=
   match C with
-  | dy_hole => None
+  | [||] => None
   | dy_binde _ _ C' => ctx_M C' M
   | dy_bindm M' CM' C' =>
-    match ctx_M C' M with
-    | Some CM => Some CM
-    | None => if eq_mid M M' then Some CM' else None
-    end
+    if eqb_ID M M' then Some CM' else ctx_M C' M
   end.
 
-(* a term, a context *)
-Inductive expr_value {time : Type} :=
-  | Fun (x : expr_id) (e : tm) (C : @dy_ctx time)
-  | Func (M : mod_id) (s : st_ctx) (e : tm) (C : @dy_ctx time)
-.
-
-Inductive dy_value {time : Type} :=
-  | EVal (ev : @expr_value time)
-  | MVal (mv : @dy_ctx time)
-.
-
-Notation "Cout '[|' Cin '|]'" := (dy_plugin Cout Cin)
-                              (at level 100, Cin at next level, right associativity).
-Notation "'[||]'" := (dy_hole) (at level 100).
-
-Fixpoint In_ctx {T} (t : T) (C : @dy_ctx T) :=
-  match C with
-  | [||] => False
-  | dy_binde _ t' C' => t = t' \/ In_ctx t C'
-  | dy_bindm _ C' C'' => In_ctx t C' \/ In_ctx t C''
+Lemma inject_addr_x {T} : forall x (Cout Cin : dy_ctx T),
+  addr_x (Cin [| Cout |]) x =
+  match addr_x Cin x with
+  | Some t => Some t
+  | None => addr_x Cout x
   end.
-
-Lemma dy_plugin_assoc : forall {T} (C1 : @dy_ctx T) C2 C3, C1[| C2[| C3 |] |] = ((C1[|C2|])[|C3|]).
 Proof.
-  induction C1; eauto; 
-  intros; simpl; try rewrite IHC1; eauto.
-  rewrite IHC1_2. eauto.
+  induction Cin; ii; ss. des_goal; eauto.
 Qed.
 
-Fixpoint dy_to_st {T} (C : @dy_ctx T) :=
+Lemma inject_ctx_M {T} : forall M (Cout Cin : dy_ctx T),
+  ctx_M (Cin [| Cout |]) M =
+  match ctx_M Cin M with
+  | Some CM => Some CM
+  | None => ctx_M Cout M
+  end.
+Proof.
+  induction Cin; ii; ss. des_goal; eauto.
+Qed.
+
+(* Auxiliary definition to aid proofs *)
+Fixpoint st_level (C : st_ctx) :=
   match C with
-  | ([||]) => st_hole
+  | [[||]] => 0
+  | st_binde _ C' => S (st_level C')
+  | st_bindm _ C' C'' => S (Nat.max (st_level C') (st_level C''))
+  end.
+
+Fixpoint dy_level {T} (C : dy_ctx T) :=
+  match C with
+  | [||] => 0
+  | dy_binde _ _ C' => S (dy_level C')
+  | dy_bindm _ C' C'' => S (Nat.max (dy_level C') (dy_level C''))
+  end.
+
+Fixpoint dy_to_st {T} (C : dy_ctx T) :=
+  match C with
+  | [||] => [[||]]
   | dy_binde x _ C' => st_binde x (dy_to_st C')
   | dy_bindm M CM C' => st_bindm M (dy_to_st CM) (dy_to_st C')
   end.
 
-Lemma in_plugin_iff :
-  forall {T} (t : T) (Cout Cin : @dy_ctx T),
-    In_ctx t (Cout[|Cin|]) <-> (In_ctx t Cout \/ In_ctx t Cin).
+Lemma dy_to_st_inject {T} (Cout : dy_ctx T) :
+  forall Cin, dy_to_st (Cin [|Cout|]) = (dy_to_st Cin [[|dy_to_st Cout|]]).
 Proof.
-  intros. revert Cin.
-  induction Cout; intros; split; simpl; intros H; 
-  try rewrite IHCout in H;
-  try rewrite IHCout2 in H;
-  try rewrite IHCout;
-  try rewrite IHCout2;
-  try destruct H as [? | [? | ?]];
-  try destruct H as [[? | ?] | ?];
-  eauto.
-  destruct H; try assumption; inversion H.
+  induction Cin; ss; rw; eauto.
 Qed.
 
-Lemma dy_to_st_plugin :
-  forall {T} (Cout : @dy_ctx T) Cin,
-    dy_to_st (Cout[|Cin|]) = st_plugin (dy_to_st Cout) (dy_to_st Cin).
+Lemma st_dy_level_eq {T} :
+  forall (C : dy_ctx T), dy_level C = st_level (dy_to_st C).
 Proof.
-  induction Cout; intros; simpl; try rewrite IHCout; eauto.
-  rewrite IHCout2. eauto.
-Qed. 
+  induction C; simpl; eauto.
+Qed.
 
-Lemma mod_is_static_none : forall {T} (dC : @dy_ctx T) (M : mod_id),
+Lemma mod_is_static_none : forall {T} (dC : dy_ctx T) (M : ID),
   (ctx_M dC M = None <-> st_ctx_M (dy_to_st dC) M = None).
 Proof. 
-  intros. repeat split. 
-  - induction dC; simpl; eauto.
-    destruct (ctx_M dC2 M). intros H; inversion H.
-    specialize (IHdC2 eq_refl). rewrite IHdC2.
-    destruct (eq_mid M M0). intros H; inversion H. eauto.
-  - induction dC; simpl; eauto.
-    destruct (st_ctx_M (dy_to_st dC2) M). intros H; inversion H.
-    specialize (IHdC2 eq_refl). rewrite IHdC2.
-    destruct (eq_mid M M0). intros H; inversion H. eauto.
+  intros. repeat split; induction dC; simpl; eauto;
+  repeat des_goal; eauto;
+  match goal with
+  | _ => let H := fresh "H" in intro H; inversion H
+  | _ => idtac
+  end.
 Qed.
 
-Lemma mod_is_static_some : forall {T} (dC : @dy_ctx T) (M : mod_id),
+Lemma mod_is_static_some : forall {T} (dC : dy_ctx T) (M : ID),
   (forall v, ctx_M dC M = Some v -> st_ctx_M (dy_to_st dC) M = Some (dy_to_st v)) /\
   (forall v, st_ctx_M (dy_to_st dC) M = Some v -> exists dv, dy_to_st dv = v /\ ctx_M dC M = Some dv).
 Proof.
-  intros; split. 
-  - induction dC; simpl; intros; eauto.
-    + inversion H.
-    + remember (ctx_M dC2 M) as v2. destruct v2.
-      specialize (IHdC2 v H). rewrite IHdC2. eauto.
-      symmetry in Heqv2. rewrite mod_is_static_none in Heqv2.
-      rewrite Heqv2. destruct (eq_mid M M0); inversion H; eauto.
-  - induction dC; simpl; intros; eauto.
-    + inversion H.
-    + remember (st_ctx_M (dy_to_st dC2) M) as v2. destruct v2.
-      specialize (IHdC2 v H). inversion IHdC2. exists x.
-      destruct H0. split. assumption. rewrite H1. eauto.
-      remember (ctx_M dC2 M) as v2. destruct v2;
-      symmetry in Heqv2; rewrite <- mod_is_static_none in Heqv2.
-      rewrite Heqv2 in Heqv0. inversion Heqv0.
-      destruct (eq_mid M M0). inversion H.
-      exists dC1. eauto. inversion H.
+  intros; split; induction dC; simpl; intros; eauto; clarify;
+  repeat des_goal; clarify; eauto.
 Qed.
 
-Class Eq T : Type :=
-{
-  eqb : T -> T -> bool;
-  eqb_eq : forall (t t' : T), eqb t t' = true <-> t = t';
-  eqb_neq : forall (t t' : T), eqb t t' = false <-> t <> t'
-}.
+(* More semantic domains *)
+Inductive expr_value T :=
+  | Fun (x : ID) (e : tm) (C : dy_ctx T)
+  | Func (M : ID) (s : st_ctx) (e : tm) (C : dy_ctx T)
+.
 
-Fixpoint eq_ctx {T} `{Eq T} (C1 : @dy_ctx T) (C2 : @dy_ctx T) :=
+Arguments Fun {T}.
+Arguments Func {T}.
+
+Inductive dy_value T :=
+  | EVal (ev : expr_value T)
+  | MVal (mv : dy_ctx T)
+.
+
+Arguments EVal {T}.
+Arguments MVal {T}.
+
+Definition memory T := list (T * expr_value T).
+
+Definition update_m {T X} m (t : T) (x : X) := (t, x) :: m.
+
+Definition empty_mem {T} : list T := [].
+
+Notation "p '!->' v ';' mem" := (update_m mem p v)
+                              (at level 100, v at next level, right associativity).
+
+Inductive config T :=
+  | Cf (e : tm) (C : dy_ctx T) (m : memory T) (t : T)
+  | Rs (V : dy_value T) (m : memory T) (t : T)
+.
+
+Arguments Cf {T}.
+Arguments Rs {T}.
+
+(* memory reads *)
+Fixpoint read {T} `{Eq T} (m : memory T) (t : T) :=
+  match m with
+  | [] => None
+  | (t', v) :: m' =>
+    if eqb t' t then Some v else read m' t
+  end.
+
+Lemma read_top {T }`{Eq T} :
+  forall a b t,
+  read (a ++ b) t = 
+  match read a t with
+  | None => read b t
+  | Some _ => read a t
+  end.
+Proof.
+  induction a; ii; ss;
+  repeat des_goal; repeat des_hyp; clarify;
+  repeat rw; reflexivity.
+Qed.
+
+Definition same {T} `{Eq T} (m : memory T) (m' : memory T) :=
+  forall t v, Some v = read m t <-> Some v = read m' t.
+
+Fixpoint aread {T} `{Eq T} (m : memory T) (t : T) :=
+  match m with
+  | [] => []
+  | (t', v) :: m' =>
+    let tl := aread m' t in
+    if eqb t' t then v :: tl else tl
+  end.
+
+Definition asame {T} `{Eq T} (m : memory T) (m' : memory T) :=
+  forall t v, In v (aread m t) <-> In v (aread m' t).
+
+(* Definitions for the (finite) supports *)
+Fixpoint supp_C {T} (C : dy_ctx T) (t : T) :=
+  match C with
+  | [||] => False
+  | dy_binde _ t' C' => t = t' \/ supp_C C' t
+  | dy_bindm _ C' C'' => supp_C C' t \/ supp_C C'' t
+  end.
+
+Definition supp_v {T} (v : expr_value T) :=
+  match v with
+  | Fun _ _ C
+  | Func _ _ _ C => supp_C C
+  end.
+
+Definition supp_V {T} (V : dy_value T) :=
+  match V with
+  | EVal ev => supp_v ev
+  | MVal mv => supp_C mv
+  end.
+
+Fixpoint supp_m {T} (m : memory T) (t : T) :=
+  match m with
+  | [] => False
+  | (t', v) :: m' =>
+    t = t' \/ supp_v v t \/ supp_m m' t
+  end.
+
+Definition supp_ρ {T} (ρ : config T) (t : T) :=
+  match ρ with
+  | Cf _ C m time => supp_C C t \/ supp_m m t \/ time = t
+  | Rs V m time => supp_V V t \/ supp_m m t \/ time = t
+  end.
+
+(* Translation of timestamps *)
+Fixpoint trans_C {T T'} (α : T -> T') (C : dy_ctx T) :=
+  match C with
+  | [||] => [||]
+  | dy_binde x t C' => dy_binde x (α t) (trans_C α C')
+  | dy_bindm M CM C' => dy_bindm M (trans_C α CM) (trans_C α C')
+  end.
+
+Definition trans_v {T T'} (α : T -> T') (v : expr_value T) :=
+  match v with
+  | Fun x e C => Fun x e (trans_C α C)
+  | Func M s e C => Func M s e (trans_C α C)
+  end.
+
+Definition trans_V {T T'} (α : T -> T') (V : dy_value T) :=
+  match V with
+  | EVal v => EVal (trans_v α v)
+  | MVal C => MVal (trans_C α C)
+  end.
+
+Fixpoint trans_m_aux {CT AT} `{Eq CT} (α : CT -> AT) (m : memory CT) (seen : list CT) :=
+  match m with
+  | [] => []
+  | (t, v) :: m' =>
+    if Inb t seen then trans_m_aux α m' seen else
+    (α t, trans_v α v) :: trans_m_aux α m' (t :: seen)
+  end.
+
+Definition trans_m {CT AT} `{Eq CT} (α : CT -> AT) (m : memory CT) : memory AT :=
+  trans_m_aux α m [].
+
+Definition trans_ρ {CT AT} `{Eq CT} (α : CT -> AT) (ρ : config CT) :=
+  match ρ with
+  | Cf e C m t => Cf e (trans_C α C) (trans_m α m) (α t)
+  | Rs V m t => Rs (trans_V α V) (trans_m α m) (α t)
+  end.
+
+(* Lemmas on translation *)
+Lemma trans_C_inject {T TT} (α : T -> TT) :
+  forall (C1 C2 : dy_ctx T),
+    trans_C α (C1 [|C2|]) = (trans_C α C1 [|trans_C α C2|]).
+Proof.
+  induction C1; ii; ss; rw; exact eq_refl.
+Qed.
+
+Lemma aread_in {T} `{Eq T} :
+  forall (m : memory T) t v, In v (aread m t) <-> In (t, v) m.
+Proof.
+  induction m; intros; split; intros IN; simpl in *;
+  repeat des_hyp;
+  repeat des_goal;
+  repeat match goal with
+  | H : _ \/ _ |- _ => destruct H
+  end; clarify;
+  try rewrite eqb_eq in *;
+  try rewrite IHm in *;
+  clarify; eauto.
+  rewrite eqb_neq in *. contradict.
+Qed.
+
+Lemma trans_m_aux_read {CT AT} `{Eq CT} `{Eq AT} (α : CT -> AT) 
+  (INJ : forall x y, α x = α y -> x = y) :
+  forall m abs_t abs_v seen,
+  Some abs_v = read (trans_m_aux α m seen) abs_t <->
+  (exists t v, ~ In t seen /\ Some v = read m t /\ α t = abs_t /\ trans_v α v = abs_v).
+Proof.
+  induction m; intros; split; intros IN; simpl in *;
+  repeat match goal with
+  | H : exists _, _ |- _ => destruct H as [t [v ?]]
+  | H : _ /\ _ |- _ => destruct H
+  end; clarify;
+  repeat des_goal; repeat des_hyp;
+  try rewrite eqb_eq in *;
+  match goal with
+  | H : _ |- _ => apply INJ in H
+  | _ => idtac
+  end; clarify;
+  try rewrite t_refl in *;
+  try rewrite Inb_eq in *;
+  try rewrite Inb_neq in *; clarify. try contradict; eauto.
+  - rewrite IHm in IN.
+    destruct IN as [t [v [IN [? [? ?]]]]]; clarify.
+    exists t. exists v. repeat split; try assumption.
+    des_goal; try rewrite eqb_eq in *; subst; try contradict; eauto.
+  - exists c. exists e. rewrite t_refl. eauto.
+  - rewrite IHm in IN.
+    destruct IN as [t [v [IN [? [? ?]]]]]; clarify. simpl in IN.
+    exists t. exists v. repeat split; eauto.
+    des_goal; try rewrite eqb_eq in *; subst; try contradict; eauto.
+  - rewrite IHm. exists t. exists v. eauto.
+  - rewrite IHm. exists t. exists v.
+    rewrite <- Inb_neq in *. simpl. repeat rw. eauto.
+Qed.
+
+Lemma trans_m_aux_aread {CT AT} `{Eq CT} (α : CT -> AT) :
+  forall m abs_t abs_v seen,
+  In (abs_t, abs_v) (trans_m_aux α m seen) <->
+  (exists t v, ~ In t seen /\ Some v = read m t /\ α t = abs_t /\ trans_v α v = abs_v).
+Proof.
+  induction m; intros; split; intros IN; simpl in *;
+  repeat match goal with
+  | H : exists _, _ |- _ => destruct H as [t [v ?]]
+  | H : _ /\ _ |- _ => destruct H
+  end; clarify;
+  repeat des_goal; repeat des_hyp;
+  try rewrite eqb_eq in *;
+  try rewrite t_refl in *; clarify;
+  try rewrite Inb_eq in *; try contradict; eauto.
+  - rewrite IHm in IN.
+    destruct IN as [t [v [IN [READ [TRANSt TRANSv]]]]].
+    exists t. exists v. repeat split; try assumption.
+    des_goal; try rewrite eqb_eq in *; subst; try contradict; eauto.
+  - destruct IN as [IN|IN].
+    clarify. exists c. exists e. rewrite t_refl. rewrite <- Inb_neq. eauto.
+    rewrite IHm in IN.
+    destruct IN as [t [v [IN [READ [TRANSt TRANSv]]]]].
+    exists t. exists v. rewrite <- Inb_neq in *. simpl in *.
+    repeat des_hyp; clarify; eauto.
+  - rewrite IHm. exists t. exists v. eauto.
+  - right. rewrite IHm. exists t. exists v.
+    rewrite <- Inb_neq in *. simpl.
+    repeat des_hyp; clarify; eauto.
+Qed.
+
+Lemma trans_m_read {CT AT} `{Eq CT} `{Eq AT} (α : CT -> AT) 
+  (INJ : forall x y, α x = α y -> x = y) :
+  forall (m : memory CT) t v,
+  Some v = read (trans_m α m) t <->
+  (exists t' v', Some v' = read m t' /\ α t' = t /\ trans_v α v' = v).
+Proof.
+  induction m; intros; split; intros IN; simpl in *;
+  repeat match goal with
+  | H : exists _, _ |- _ => destruct H as [t [v ?]]
+  | H : _ /\ _ |- _ => destruct H
+  end; clarify;
+  repeat des_goal; repeat des_hyp;
+  try rewrite eqb_eq in *;
+  match goal with
+  | H : _ |- _ => apply INJ in H
+  | _ => idtac
+  end; clarify;
+  try rewrite t_refl in *;
+  try rewrite Inb_eq in *;
+  try rewrite Inb_neq in *; clarify. try contradict; eauto.
+  - destruct IN as [? [? [? ?]]]; clarify.
+  - unfold trans_m in IN. simpl in IN.
+    des_hyp. exists c. exists e. rewrite t_refl. rewrite eqb_eq in *.
+    clarify. eauto.
+    rewrite trans_m_aux_read in IN; eauto.
+    destruct IN as [t' [v' [IN [READ [TRANSt TRANSv]]]]].
+    exists t'. exists v'. repeat split; eauto.
+    des_goal; try rewrite eqb_eq in *; subst; eauto.
+    exfalso. apply IN. simpl. eauto.
+  - unfold trans_m. simpl. 
+    des_goal; try rewrite eqb_eq in *; subst;
+    try rewrite trans_m_aux_read; eauto;
+    destruct IN as [t' [v' [READ [TRANSt TRANSv]]]];
+    try apply INJ in TRANSt; subst; try rewrite t_refl in *. clarify.
+    exists t'. exists v'. 
+    des_hyp; 
+    try rewrite eqb_eq in *; clarify;
+    try rewrite t_refl in *; clarify;
+    repeat rewrite eqb_neq in *.
+    simpl. repeat split; eauto.
+    red; intros contra; destruct contra; eauto.
+Qed.
+
+Lemma trans_m_aread {CT AT} `{Eq CT} `{Eq AT} (α : CT -> AT) :
+  forall (m : memory CT) t v,
+  In v (aread (trans_m α m) t) <->
+  (exists t' v', Some v' = read m t' /\ α t' = t /\ trans_v α v' = v).
+Proof.
+  induction m; intros; split; intros IN;
+  try (simpl in IN; contradict);
+  try (destruct IN as [t' [v' [? [? ?]]]]; clarify);
+  unfold trans_m in *; simpl in *; repeat des_hyp; clarify;
+  match goal with
+  | _ => simpl in *; rewrite t_refl in *; clarify
+  | _ => idtac
+  end;
+  try rewrite eqb_eq in *; 
+  try rewrite aread_in in *;
+  subst; simpl; eauto.
+  - destruct IN as [IN|IN].
+    subst. exists c. exists e. rewrite t_refl; eauto.
+    rewrite trans_m_aux_aread in IN.
+    destruct IN as [t [v' [IN [? [? ?]]]]].
+    rewrite <- Inb_neq in IN. simpl in IN.
+    des_hyp.
+    exists t. exists v'.
+    repeat rw. eauto.
+  - rewrite trans_m_aux_aread in IN.
+    destruct IN as [t' [v' [IN [? [? ?]]]]].
+    rewrite <- Inb_neq in IN. simpl in IN.
+    des_hyp.
+    exists t'. exists v'.
+    repeat rw. eauto.
+  - right. rewrite trans_m_aux_aread.
+    exists t'. exists v'.
+    rewrite <- Inb_neq; simpl.
+    repeat rw. eauto.
+Qed.
+
+Lemma trans_m_same {CT AT} `{Eq CT} `{Eq AT} (α : CT -> AT)
+  (INJ : forall x y, α x = α y -> x = y) :
+  forall (m m' : memory CT) (EQ : same m m'),
+    same (trans_m α m) (trans_m α m').
+Proof.
+  induction m; intros; unfold same in *;
+  intros; split; intros IN; simpl in *;
+  clarify.
+  - rewrite trans_m_read in IN; eauto.
+    destruct IN as [t' [v' [READ [TRANSt TRANSv]]]].
+    rewrite <- EQ in *. clarify.
+  - rewrite trans_m_read in *; eauto.
+    destruct IN as [t' [v' [READ [TRANSt TRANSv]]]].
+    simpl in *. repeat des_hyp; try rewrite eqb_eq in *; clarify.
+    exists t'. exists e. repeat split; eauto.
+    rewrite <- EQ. rewrite t_refl. eauto.
+    exists t'. exists v'. repeat split; eauto.
+    rewrite <- EQ. repeat rw. eauto.
+  - rewrite trans_m_read in *; eauto.
+    destruct IN as [t' [v' [READ [TRANSt TRANSv]]]].
+    simpl in *. repeat des_goal; try rewrite eqb_eq in *; clarify.
+    exists t'. exists v'. repeat split; eauto.
+    rewrite EQ. eauto.
+Qed.
+
+Lemma trans_m_asame {CT AT} `{Eq CT} `{Eq AT} (α : CT -> AT) :
+  forall (m m' : memory CT) (EQ : same m m'),
+    asame (trans_m α m) (trans_m α m').
+Proof.
+  induction m; intros; unfold same in EQ;
+  unfold asame; intros; split; intros IN; simpl in *;
+  clarify.
+  - rewrite trans_m_aread in IN.
+    destruct IN as [? [? [contra [? ?]]]].
+    rewrite <- EQ in contra. inversion contra.
+  - rewrite trans_m_aread in *.
+    destruct IN as [t' [v' [? [? ?]]]].
+    simpl in *. repeat des_hyp; clarify.
+    exists t'. exists e. repeat split; try reflexivity.
+    rewrite <- EQ. repeat rw. eauto.
+    exists t'. exists v'. repeat split; try reflexivity.
+    rewrite <- EQ. repeat rw. eauto.
+  - rewrite trans_m_aread in *.
+    destruct IN as [t' [v' [READ [? ?]]]].
+    simpl in *. rewrite <- EQ in READ.
+    exists t'. exists v'. eauto.
+Qed.
+
+Lemma trans_C_addr :
+  forall {CT AT} (α : CT -> AT) C x,
+    addr_x (trans_C α C) x = 
+      match addr_x C x with 
+      | None => None 
+      | Some addr => Some (α addr)
+      end.
+Proof.
+  induction C; eauto.
+  intros. simpl.
+  des_goal; eauto.
+Qed.
+
+Lemma trans_C_ctx_M :
+  forall {CT AT} C (α : CT -> AT) M,
+    ctx_M (trans_C α C) M =
+      match ctx_M C M with
+      | None => None
+      | Some CM => Some (trans_C α CM)
+      end.
+Proof.
+  induction C; ii; ss.
+  des_goal; eauto.
+Qed.
+
+Fixpoint eq_C {T} eqb (C1 C2 : dy_ctx T) :=
   match C1, C2 with
   | [||], [||] => true
   | dy_binde x1 t1 C1', dy_binde x2 t2 C2' =>
-    eq_eid x1 x2 && eqb t1 t2 && eq_ctx C1' C2'
+    eqb_ID x1 x2 && eqb t1 t2 && eq_C eqb C1' C2'
   | dy_bindm M1 C1' C1'', dy_bindm M2 C2' C2'' =>
-    eq_mid M1 M2 && eq_ctx C1' C2' && eq_ctx C1'' C2''
+    eqb_ID M1 M2 && eq_C eqb C1' C2' && eq_C eqb C1'' C2''
   | _, _ => false
   end.
 
-Lemma eq_ctx_eq : forall {T} `{Eq T} (C C' : dy_ctx),
-  eq_ctx C C' = true <-> C = C'.
+Lemma ctx_refl {T} eqb (t_refl : forall t, eqb t t = true) : 
+  forall (C : dy_ctx T), eq_C eqb C C = true.
 Proof.
-  intros. rename H into ET. revert C'.
-  induction C; destruct C'; split; intros H; inversion H; try reflexivity;
-  try (assert (x = x0);
-    [rewrite <- eq_eid_eq | idtac];
-    destruct (eq_eid x x0); inversion H1; eauto;
-    assert (tx = tx0);
-    [rewrite <- eqb_eq | idtac];
-    destruct (eqb tx tx0); inversion H1; eauto;
-    assert (C = C');
-    [rewrite <- IHC | idtac]; eauto; subst; reflexivity);
-  try (subst; simpl;
-    assert (eq_eid x0 x0 = true);
-    [rewrite eq_eid_eq; reflexivity | idtac];
-    assert (eqb tx0 tx0 = true);
-    [rewrite eqb_eq; reflexivity | idtac];
-    assert (eq_ctx C' C' = true);
-    [rewrite IHC; reflexivity | idtac];
-    rewrite H0; rewrite H1; rewrite H2; eauto).
-  assert (M = M0);
-  [rewrite <- eq_mid_eq; destruct (eq_mid M M0); inversion H1; eauto | idtac];
-  assert (C1 = C'1);
-  [rewrite <- IHC1; destruct (eq_mid M M0);
-   destruct (eq_ctx C1 C'1); inversion H1; eauto | idtac].
-  assert (C2 = C'2);
-  [rewrite <- IHC2; destruct (eq_mid M M0);
-   destruct (eq_ctx C1 C'1); destruct (eq_ctx C2 C'2); inversion H1; eauto | idtac];
+  induction C; simpl; try rewrite ID_refl; try rewrite t_refl;
+  try rewrite IHC; try rewrite IHC1; try rewrite IHC2; eauto.
+Qed.
+
+Definition eqb_C {T} `{Eq T} := eq_C eqb.
+
+Lemma eqb_C_eq {T} `{Eq T} :
+  forall (C C' : dy_ctx T),
+  eqb_C C C' = true <-> C = C'.
+Proof.
+  induction C; intros; unfold eqb_C in *;
+  simpl; repeat des_goal; repeat des_hyp;
+  split; intros EQ; clarify;
+  try rewrite eqb_ID_eq in *; try rewrite eqb_eq in *;
+  try rewrite IHC in *; try rewrite IHC1 in *; try rewrite IHC2 in *;
+  subst;
+  match goal with
+  | _ => reflexivity
+  | _ => rewrite eqb_neq in *; contradict
+  | _ => rewrite eqb_ID_neq in *; contradict
+  | H : eq_C eqb ?C ?C = false |- _ =>
+    let contra := fresh "contra" in
+    assert (C = C) as contra; try reflexivity;
+    match goal with
+    | RR : context[C = _] |- _ => 
+      rewrite <- RR in *; rewrite contra in *; clarify
+    end
+  end.
+Qed.
+
+#[export] Instance EqC {T} `{Eq T} : `{Eq (dy_ctx T)} := 
+  { eqb := eqb_C; eqb_eq := eqb_C_eq; }.
+
+Lemma eq_C_st_eq {T} eqb (C1 C2 : dy_ctx T) :
+  eq_C eqb C1 C2 = true -> dy_to_st C1 = dy_to_st C2.
+Proof.
+  intros EQ. revert C2 EQ.
+  induction C1; induction C2; intros; simpl; eauto; try (inversion EQ; fail);
+  simpl in EQ; repeat des_hyp;
+  repeat match goal with
+  | [H : context [eq_C eqb _ _ = true -> _] |- _] =>
+    match goal with
+    | [RR : eq_C eqb _ _ = true |- _] =>
+      apply H in RR; rewrite RR
+    end
+  | [RR : eqb_ID _ _ = true |- _] =>
+    rewrite eqb_ID_eq in RR; rewrite RR
+  end; eauto.
+Qed.
+
+Lemma eq_C_level_eq {T} eqb (C1 C2 : dy_ctx T) :
+  eq_C eqb C1 C2 = true -> dy_level C1 = dy_level C2.
+Proof.
+  intros EQ.
+  repeat rewrite st_dy_level_eq.
+  erewrite eq_C_st_eq; eauto.
+Qed.
+
+(* deletion *)
+
+Fixpoint delete {T} eqb (Cout Cin : dy_ctx T) :=
+  if eq_C eqb Cout Cin then [||]
+  else match Cin with
+  | [||] => [||]
+  | dy_binde x t Cin' =>
+    dy_binde x t (delete eqb Cout Cin')
+  | dy_bindm M Cin' Cin'' =>
+    dy_bindm M Cin' (delete eqb Cout Cin'')
+  end.
+
+Definition inject_v {T} `{Eq T} (Cout : dy_ctx T) (v : expr_value T) :=
+  match v with
+  | Fun x t C => Fun x t (C [|Cout|])
+  | Func M s t C => Func M s t (C [|Cout|])
+  end.
+
+Definition delete_v {T} eqb (Cout : dy_ctx T) (v : expr_value T) :=
+  match v with
+  | Fun x t C => Fun x t (delete eqb Cout C)
+  | Func M s t C => Func M s t (delete eqb Cout C)
+  end.
+
+Lemma inject_level_inc {T} (Cout Cin : dy_ctx T) :
+  dy_level Cout <= dy_level (Cin [| Cout |]).
+Proof.
+  induction Cin; intros; simpl; nia.
+Qed.
+
+Lemma delete_inject_eq {T} eqb (t_refl : forall t, eqb t t = true) :
+  forall (Cout Cin : dy_ctx T),
+    delete eqb Cout (Cin [|Cout|]) = Cin.
+Proof.
+  intros. revert Cout. induction Cin; simpl;
+  match goal with
+  | |- context [if _ then _ else _] =>
+    (* inductive case *)
+    intros; try rewrite IHCin; try rewrite IHCin1; try rewrite IHCin2;
+    des_goal; eauto;
+    (* search for a contradiction *)
+    match goal with
+    | [H : eq_C _ _ _ = true |- _] =>
+      apply eq_C_level_eq in H; simpl in H
+    end;
+    match goal with
+    | [H : dy_level ?Cout = _|-_] =>
+      match type of H with
+      | context [inject ?Cout ?Cin] =>
+        pose proof (inject_level_inc Cout Cin); try nia
+      end
+    end
+  | _ =>
+    (* base case *)
+    induction Cout; eauto;
+    simpl;
+    repeat rewrite ID_refl;
+    repeat rewrite t_refl;
+    repeat rewrite ctx_refl; eauto
+  end.
+Qed.
+
+(* lemmas for trans_C *)
+Lemma trans_C_id_eq {T} :
+  forall (C : dy_ctx T), trans_C id C = C.
+Proof.
+  induction C; simpl; try rewrite IHC; eauto.
+  rewrite IHC1. rewrite IHC2. reflexivity.
+Qed.
+
+Lemma eq_C_eq {T} `{Eq T} :
+  forall (C C' : @dy_ctx T),
+  eq_C eqb C C' = true <-> C = C'.
+Proof.
+  induction C; destruct C'; simpl;
+  try (split; intros contra; inversion contra; fail);
+  split; intros EQ;
+  repeat des_hyp; try reflexivity;
+  repeat match goal with
+  | [H : eqb_ID _ _ = true|-_] => rewrite eqb_ID_eq in H
+  | [H : eqb _ _ = true|-_] => rewrite eqb_eq in H
+  | [H : eq_C _ _ _ = true|-_] => 
+    try rewrite IHC in H;
+    try rewrite IHC1 in H;
+    try rewrite IHC2 in H
+  | _ => clarify
+  end; try reflexivity;
+  try rewrite ID_refl;
+  try rewrite t_refl;
+  repeat match goal with
+  | |- context[eq_C ?eqb ?C ?C] =>
+    match goal with
+    | [H : context [eq_C eqb C _ = true <-> _] |- _] =>
+      let RR := fresh "RR" in
+      assert (eq_C eqb C C = true) as RR;
+      try rewrite H; eauto; rewrite RR
+    end
+  end.
+Qed.
+
+Lemma trans_C_eq_C {CT AT} `{ECT : Eq CT} `{EAT : Eq AT} (α : CT -> AT) :
+  forall C C',
+    let eqb' t t' := eqb (α t) (α t') in
+    eq_C eqb' C C' = true <->
+    trans_C α C = trans_C α C'.
+Proof.
+  induction C; induction C'; simpl;
+  try (split; intros contra; inversion contra; eauto; fail);
+  split; intros EQ;
+  repeat des_hyp;
+  repeat match goal with
+  | [H : eqb_ID _ _ = true|-_] => 
+    rewrite eqb_ID_eq in H; rewrite H
+  | [H : eqb _ _ = true|-_] => 
+    rewrite eqb_eq in H; rewrite H
+  | [H : eq_C _ _ _ = true|-_] => 
+    try rewrite IHC in H;
+    try rewrite IHC1 in H;
+    try rewrite IHC2 in H;
+    rewrite H
+  | _ => clarify
+  end; try reflexivity;
+  try rewrite ID_refl;
+  repeat match goal with
+  | [RR : α _ = α _|-_] => rewrite RR; rewrite t_refl
+  | |- context[eq_C ?eqb' ?C ?C'] =>
+    match goal with
+    | [H : context [eq_C _ C _ = true <-> _]|-_] =>
+      let RR := fresh "RR" in
+      assert (eq_C eqb' C C' = true) as RR;
+      try rewrite H; try assumption; rewrite RR
+    | _ => fail
+    end
+  end; eauto.
+Qed.
+
+Lemma trans_C_delete {CT AT} `{ECT : Eq CT} `{EAT : Eq AT} (α : CT -> AT) :
+  forall Cout C,
+    let eqb' t t' := eqb (α t) (α t') in
+    trans_C α (delete eqb' Cout C) = delete eqb (trans_C α Cout) (trans_C α C).
+Proof.
+  intros.
+  assert (forall C', eq_C eqb' Cout C' = eq_C eqb (trans_C α Cout) (trans_C α C')) as RR.
+  { induction Cout; induction C'; eauto.
+    simpl. rewrite IHCout. eauto.
+    simpl. rewrite IHCout1. rewrite IHCout2. eauto. }
+  induction C; intros; simpl; rewrite RR; simpl;
+  des_goal; eauto;
+  try rewrite IHC;
+  try rewrite IHC1;
+  try rewrite IHC2; eauto.
+Qed.
+
+Generalizable Variables T BT AT.
+
+Fixpoint inject_ctx_mem `{Eq T} (Cout : dy_ctx T) (mem : memory T) :=
+  match mem with
+  | [] => []
+  | (t, v) :: tl =>
+    (t, inject_v Cout v) :: inject_ctx_mem Cout tl
+  end.
+
+Fixpoint delete_ctx_mem `{Eq T} eqb (Cout : dy_ctx T) (mem : memory T) :=
+  match mem with
+  | [] => []
+  | (t, v) :: tl =>
+    (t, delete_v eqb Cout v) :: delete_ctx_mem eqb Cout tl
+  end.
+
+Lemma delete_ctx_mem_eq `{Eq T} eqb (t_refl : forall t, eqb t t = true) :
+  forall (Cout : dy_ctx T) (mem : memory T),
+         delete_ctx_mem eqb Cout (inject_ctx_mem Cout mem) = mem.
+Proof.
+  induction mem; simpl; eauto.
+  repeat des_goal; clarify; rw.
+  destruct e; simpl;
+  pose proof (@delete_inject_eq T eqb) as RR;
+  rewrite RR; eauto.
+Qed.
+
+Inductive link BT AT :=
+  | BF (t : BT)
+  | AF (t : AT)
+.
+
+Arguments BF {BT AT}.
+Arguments AF {BT AT}.
+
+Definition link_eqb `{Eq BT} `{Eq AT} (t t' : link BT AT) :=
+  match t, t' with
+  | BF t, BF t' => eqb t t'
+  | AF t, AF t' => eqb t t'
+  | _, _ => false
+  end.
+
+Lemma link_eqb_eq `{Eq BT} `{Eq AT} :
+  forall (t t' : link BT AT), link_eqb t t' = true <-> t = t'.
+Proof.
+  intros.
+  destruct t; destruct t'; simpl; split; intros EQ; 
+  try rewrite eqb_eq in *;
+  try inversion EQ;
   subst; eauto.
-  subst; simpl.
-  assert (eq_mid M0 M0 = true);
-  [rewrite eq_mid_eq; reflexivity | idtac];
-  assert (eq_ctx C'1 C'1 = true);
-  [rewrite IHC1; reflexivity | idtac];
-  assert (eq_ctx C'2 C'2 = true);
-  [rewrite IHC2; reflexivity | idtac];
-  rewrite H0; rewrite H1; rewrite H2; eauto.
 Qed.
 
-Lemma eq_ctx_neq : forall {T} `{Eq T} (C C' : dy_ctx),
-  eq_ctx C C' = false <-> C <> C'.
+#[export] Instance link_eq `{Eq BT} `{Eq AT} : Eq (link BT AT) :=
+  {
+    eqb := link_eqb;
+    eqb_eq := link_eqb_eq;
+  }.
+
+Fixpoint filter_ctx_bf {BT AT} (C : dy_ctx (link BT AT)) :=
+  match C with
+  | [||] => [||]
+  | dy_binde x t C' =>
+    match t with
+    | BF t => dy_binde x t (filter_ctx_bf C')
+    | AF t => filter_ctx_bf C'
+    end
+  | dy_bindm M C' C'' => dy_bindm M (filter_ctx_bf C') (filter_ctx_bf C'')
+  end.
+
+Fixpoint filter_ctx_af {BT AT} (C : dy_ctx (link BT AT)) :=
+  match C with
+  | [||] => [||]
+  | dy_binde x t C' =>
+    match t with
+    | AF t => dy_binde x t (filter_ctx_af C')
+    | BF t => filter_ctx_af C'
+    end
+  | dy_bindm M C' C'' => dy_bindm M (filter_ctx_af C') (filter_ctx_af C'')
+  end.
+
+Definition filter_v_bf {BT AT} (v : expr_value (link BT AT)) :=
+  match v with
+  | Fun x e C => Fun x e (filter_ctx_bf C)
+  | Func M s e C => Func M s e (filter_ctx_bf C)
+  end.
+
+Definition filter_v_af {BT AT} (v : expr_value (link BT AT)) :=
+  match v with
+  | Fun x e C => Fun x e (filter_ctx_af C)
+  | Func M s e C => Func M s e (filter_ctx_af C)
+  end.
+
+Fixpoint filter_mem_bf {BT AT} (mem : memory (link BT AT)) :=
+  match mem with
+  | [] => []
+  | (AF _, _) :: tl => filter_mem_bf tl
+  | (BF t, v) :: tl => (t, filter_v_bf v) :: filter_mem_bf tl
+  end.
+
+Fixpoint filter_mem_af {BT AT} (mem : memory (link BT AT)) :=
+  match mem with
+  | [] => []
+  | (AF t, v) :: tl => (t, filter_v_af v) :: filter_mem_af tl
+  | (BF _, _) :: tl => filter_mem_af tl
+  end.
+
+Fixpoint lift_ctx_bf {BT AT} C : dy_ctx (link BT AT) :=
+  match C with
+  | [||] => [||]
+  | dy_binde x t C' => dy_binde x (BF t) (lift_ctx_bf C')
+  | dy_bindm M C' C'' => dy_bindm M (lift_ctx_bf C') (lift_ctx_bf C'')
+  end.
+
+Definition lift_v_bf {BT AT} v : expr_value (link BT AT) :=
+  match v with
+  | Fun x e C => Fun x e (lift_ctx_bf C)
+  | Func M s e C => Func M s e (lift_ctx_bf C)
+  end.
+
+Fixpoint lift_mem_bf {BT AT} m : memory (link BT AT) :=
+  match m with
+  | [] => []
+  | (t, v) :: tl => (BF t, lift_v_bf v) :: lift_mem_bf tl
+  end.
+
+Fixpoint lift_ctx_af {BT AT} C : dy_ctx (link BT AT) :=
+  match C with
+  | [||] => [||]
+  | dy_binde x t C' => dy_binde x (AF t) (lift_ctx_af C')
+  | dy_bindm M C' C'' => dy_bindm M (lift_ctx_af C') (lift_ctx_af C'')
+  end.
+
+Definition lift_v_af {BT AT} v : expr_value (link BT AT) :=
+  match v with
+  | Fun x e C => Fun x e (lift_ctx_af C)
+  | Func M s e C => Func M s e (lift_ctx_af C)
+  end.
+
+Fixpoint lift_mem_af {BT AT} m : memory (link BT AT) :=
+  match m with
+  | [] => []
+  | (t, v) :: tl => (AF t, lift_v_af v) :: lift_mem_af tl
+  end.
+
+Lemma read_filter_bf `{Eq BT} `{Eq AT} :
+  forall (m : memory (link BT AT)) (t : BT) (v : expr_value BT),
+    Some v = read (filter_mem_bf m) t <->
+    exists v', v = filter_v_bf v' /\ Some v' = read m (BF t).
 Proof.
-  intros; split; intros.
-  - red; intros contra. rewrite <- eq_ctx_eq in contra.
-    rewrite contra in H0. inversion H0.
-  - destruct (eq_ctx C C') eqn:EQ; try reflexivity.
-    rewrite eq_ctx_eq in EQ. apply H0 in EQ. inversion EQ.
+  induction m; ii;
+  split; intros READ; ss;
+  repeat des_goal; repeat des_hyp; des;
+  try rewrite eqb_eq in *;
+  try rewrite eqb_neq in *;
+  try rewrite link_eqb_eq in *;
+  clarify; eauto;
+  try rewrite <- aread_in in *;
+  first [ rewrite IHm in READ; des; eauto 
+        | try right; rewrite IHm; exists v'; eauto
+        | ss; rewrite eqb_neq in *; contradict].
 Qed.
 
-Lemma plugin_ctx_addr_x :
-  forall {T} `{Eq T} x (Cout : @dy_ctx T) (Cin : @dy_ctx T),
-    match addr_x Cin x with
-    | Some t => addr_x (Cout[|Cin|]) x = Some t
-    | None => True
-    end.
+Lemma aread_filter_bf `{Eq BT} `{Eq AT} :
+  forall (m : memory (link BT AT)) (t : BT) (v : expr_value BT),
+    In v (aread (filter_mem_bf m) t) <->
+    exists v', v = filter_v_bf v' /\ In v' (aread m (BF t)).
 Proof.
-  intros. revert Cin.
-  induction Cout; intros; 
-  destruct (addr_x Cin x) eqn:ADDR; simpl; eauto;
-  try (specialize (IHCout Cin); rewrite ADDR in IHCout;
-      rewrite IHCout; eauto).
-  specialize (IHCout2 Cin); rewrite ADDR in IHCout2; rewrite IHCout2; eauto.
+  induction m; ii; rewrite aread_in in *;
+  split; intros READ; ss;
+  repeat des_goal; repeat des_hyp; des;
+  try rewrite eqb_eq in *; 
+  try rewrite link_eqb_eq in *;
+  clarify; eauto;
+  try rewrite <- aread_in in *;
+  first [ rewrite IHm in READ; des; eauto 
+        | try right; rewrite IHm; exists v'; eauto
+        | ss; rewrite eqb_neq in *; contradict].
 Qed.
 
-Lemma plugin_ctx_ctx_M :
-  forall {T} `{Eq T} M (Cout : @dy_ctx T) (Cin : @dy_ctx T),
-    match ctx_M Cin M with
-    | Some CM => ctx_M (Cout[|Cin|]) M = Some CM
-    | None => True
-    end.
+Lemma read_filter_af `{Eq BT} `{Eq AT} :
+  forall (m : memory (link BT AT)) (t : AT) (v : expr_value AT),
+    Some v = read (filter_mem_af m) t <->
+    exists v', v = filter_v_af v' /\ Some v' = read m (AF t).
 Proof.
-  intros. revert Cin.
-  induction Cout; intros;
-  destruct (ctx_M Cin M) eqn:CTX; simpl; eauto;
-  try (specialize (IHCout Cin); rewrite CTX in IHCout;
-      rewrite IHCout; eauto).
-  specialize (IHCout2 Cin); rewrite CTX in IHCout2; rewrite IHCout2; eauto.
+  induction m; ii;
+  split; intros READ; ss;
+  repeat des_goal; repeat des_hyp; des;
+  try rewrite eqb_eq in *;
+  try rewrite eqb_neq in *;
+  try rewrite link_eqb_eq in *;
+  clarify; eauto;
+  try rewrite <- aread_in in *;
+  first [ rewrite IHm in READ; des; eauto 
+        | try right; rewrite IHm; exists v'; eauto
+        | ss; rewrite eqb_neq in *; contradict].
 Qed.
+
+Lemma aread_filter_af `{Eq BT} `{Eq AT} :
+  forall (m : memory (link BT AT)) (t : AT) (v : expr_value AT),
+    In v (aread (filter_mem_af m) t) <->
+    exists v', v = filter_v_af v' /\ In v' (aread m (AF t)).
+Proof.
+  induction m; ii; rewrite aread_in in *;
+  split; intros READ; ss;
+  repeat des_goal; repeat des_hyp; des;
+  try rewrite eqb_eq in *; 
+  try rewrite link_eqb_eq in *;
+  clarify; eauto;
+  try rewrite <- aread_in in *;
+  first [ rewrite IHm in READ; des; eauto 
+        | try right; rewrite IHm; exists v'; eauto
+        | ss; rewrite eqb_neq in *; contradict].
+Qed.
+
+Lemma read_delete `{Eq T} eqb :
+  forall (m : memory T) (Cout : dy_ctx T) t v,
+    Some v = read (delete_ctx_mem eqb Cout m) t <->
+    exists v', v = delete_v eqb Cout v' /\ Some v' = read m t.
+Proof.
+  induction m; intros; ss; split; intros READ;
+  des; try contradict; repeat des_hyp; des; ss; 
+  try rewrite eqb_eq in *; clarify;
+  try rewrite t_refl; ss; eauto;
+  first [ rewrite IHm in READ; des; eauto
+        | try right; rewrite IHm; exists v'; eauto].
+Qed.
+
+Lemma aread_delete `{Eq T} eqb :
+  forall (m : memory T) (Cout : dy_ctx T) t v,
+    In v (aread (delete_ctx_mem eqb Cout m) t) <->
+    exists v', v = delete_v eqb Cout v' /\ In v' (aread m t).
+Proof.
+  induction m; intros; ss; split; intros READ;
+  des; try contradict; repeat des_hyp; des; ss; 
+  try rewrite eqb_eq in *; clarify;
+  try rewrite t_refl; ss; eauto;
+  first [ rewrite IHm in READ; des; eauto
+        | try right; rewrite IHm; exists v'; eauto].
+Qed.
+
+Definition link_mem `{Eq BT} `{Eq AT}
+  (bmem : memory BT) (Cout : dy_ctx BT)
+  (amem : memory AT) : (memory (link BT AT)) :=
+  (inject_ctx_mem (lift_ctx_bf Cout) (lift_mem_af amem)) ++ 
+  (lift_mem_bf bmem).
+
+Fixpoint map_m {T1 T2} (f : T1 -> T2) (m : memory T1) :=
+  match m with
+  | [] => []
+  | (t, Fun x e C) :: tl =>
+    (f t, Fun x e (trans_C f C)) :: map_m f tl
+  | (t, Func M s e C) :: tl =>
+    (f t, Func M s e (trans_C f C)) :: map_m f tl
+  end.
+
+Lemma inject_ctx_mem_app `{Eq T} :
+  forall a b (C : dy_ctx T),
+  inject_ctx_mem C (a ++ b) = inject_ctx_mem C a ++ inject_ctx_mem C b.
+Proof.
+  induction a; ii; ss. des_goal. rw. eauto.
+Qed.
+
+Lemma lift_mem_bf_app `{Eq BT} `{Eq AT} :
+  forall a b,
+  (lift_mem_bf (a ++ b) : memory (link BT AT)) =
+  lift_mem_bf a ++ lift_mem_bf b.
+Proof.
+  induction a; ii; ss. des_goal. rw. eauto.
+Qed.
+
+Lemma lift_mem_af_app `{Eq BT} `{Eq AT} :
+  forall a b,
+  (lift_mem_af (a ++ b) : memory (link BT AT)) =
+  lift_mem_af a ++ lift_mem_af b.
+Proof.
+  induction a; ii; ss. des_goal. rw. eauto.
+Qed.
+
+Lemma lift_twice `{Eq T1} `{Eq T2} `{Eq T3} :
+  forall C,
+  let f (t : link T1 (link T2 T3)) : link (link T1 T2) T3 :=
+    match t with
+    | BF t1 => BF (BF t1)
+    | AF (BF t2) => BF (AF t2)
+    | AF (AF t3) => AF t3
+    end in
+  trans_C f (lift_ctx_af (lift_ctx_af C)) = lift_ctx_af C.
+Proof.
+  induction C; ii; ss; subst f; repeat rw; eauto.
+Qed.
+
+Lemma lift_once `{Eq T1} `{Eq T2} `{Eq T3} :
+  forall C,
+  let f (t : link T1 (link T2 T3)) : link (link T1 T2) T3 :=
+    match t with
+    | BF t1 => BF (BF t1)
+    | AF (BF t2) => BF (AF t2)
+    | AF (AF t3) => AF t3
+    end in
+  trans_C f (lift_ctx_af (lift_ctx_bf C)) = lift_ctx_bf (lift_ctx_af C).
+Proof.
+  induction C; ii; ss; subst f; repeat rw; eauto.
+Qed.
+
+Lemma link_ctx_assoc `{Eq T1} `{Eq T2} `{Eq T3} :
+  forall C3 C2 C1,
+  let f (t : link T1 (link T2 T3)) : link (link T1 T2) T3 :=
+    match t with
+    | BF t1 => BF (BF t1)
+    | AF (BF t2) => BF (AF t2)
+    | AF (AF t3) => AF t3
+    end in
+  trans_C f
+    (lift_ctx_af (lift_ctx_af C3 [|lift_ctx_bf C2|]) [|lift_ctx_bf C1|]) =
+  (lift_ctx_af C3 [|lift_ctx_bf (lift_ctx_af C2 [|lift_ctx_bf C1|])|]).
+Proof.
+  induction C3; ii; ss; repeat rw;
+  first [f_equal; apply lift_twice | idtac].
+  revert C2 C1.
+  induction C2; ii; ss; repeat rw;
+  first [f_equal; apply lift_once | idtac].
+  induction C1; ii; ss; repeat rw; eauto.
+Qed.
+
+Ltac des_v :=
+  match goal with
+  | v : expr_value _ |- _ => destruct v; ss; clarify
+  end.
+
+Lemma link_mem_assoc `{Eq T1} `{Eq T2} `{Eq T3} :
+  forall m1 C1 m2 C2 m3,
+  let f (t : link T1 (link T2 T3)) : link (link T1 T2) T3 :=
+    match t with
+    | BF t1 => BF (BF t1)
+    | AF (BF t2) => BF (AF t2)
+    | AF (AF t3) => AF t3
+    end in
+  map_m f (link_mem m1 C1 (link_mem m2 C2 m3)) =
+  link_mem (link_mem m1 C1 m2) ((lift_ctx_af C2)[|lift_ctx_bf C1|]) m3.
+Proof.
+  ii.
+  unfold link_mem.
+  repeat (rewrite lift_mem_af_app 
+  || rewrite inject_ctx_mem_app 
+  || rewrite lift_mem_bf_app
+  || rewrite <- app_assoc).
+  revert m3 m2 C2 m1 C1.
+  induction m3; ii; ss.
+  revert m2 m1 C1.
+  induction m2; ii; ss.
+  - induction m1; ii; ss.
+    repeat des_goal; clarify; des_v;
+    rw; repeat f_equal;
+    subst f;
+    pose proof (@link_ctx_assoc T1 _ T2 _ T3 _ ([||]) ([||]) C0); ss.
+  - repeat des_goal; clarify; des_v;
+    rw; repeat f_equal;
+    subst f; pose proof (link_ctx_assoc ([||]) C0 C1); ss.
+  - repeat des_goal; clarify; des_v;
+    rw; repeat f_equal;
+    subst f; rewrite link_ctx_assoc; eauto.
+Qed.
+
+Lemma filter_lift_eq_af {BT AT} :
+  forall (C : dy_ctx AT),
+    filter_ctx_af (@lift_ctx_af BT AT C) = C.
+Proof.
+  induction C; simpl; repeat rw; eauto.
+Qed.
+
+Lemma filter_lift_eq_bf {BT AT} :
+  forall (C : dy_ctx BT),
+    filter_ctx_bf (@lift_ctx_bf BT AT C) = C.
+Proof.
+  induction C; simpl; repeat rw; eauto.
+Qed.
+
+Lemma filter_delete_eq `{Eq BT} `{Eq AT} (Cout : dy_ctx BT) 
+  eqb (t_refl : forall t, eqb t t = true) :
+  forall bmem amem,
+  filter_mem_af
+    (delete_ctx_mem eqb (lift_ctx_bf Cout)
+    (link_mem bmem Cout amem)) = amem.
+Proof.
+  induction amem; unfold link_mem;
+  ss; repeat des_goal; unfold delete_v;
+  ss; repeat des_goal; try des_v.
+  - induction bmem; simpl; eauto.
+    des_goal; clarify.
+  - rewrite delete_inject_eq; eauto.
+    rewrite filter_lift_eq_af.
+    unfold link_mem in *. rewrite IHamem; eauto.
+  - rewrite delete_inject_eq; eauto.
+    rewrite filter_lift_eq_af.
+    unfold link_mem in *. rewrite IHamem; eauto.
+Qed.
+
+Lemma link_update_m_eq `{Eq BT} `{Eq AT} (Cout : dy_ctx BT):
+  forall bmem amem (t : AT) v,
+  (AF t !-> inject_v (lift_ctx_bf Cout) (lift_v_af v);
+    (link_mem bmem Cout amem)) =
+    link_mem bmem Cout (t !-> v; amem).
+Proof.
+  intros. ss.
+Qed.
+
+Lemma lift_addr_x {BT AT} :
+  forall (C : @dy_ctx AT) x,
+    addr_x (lift_ctx_af C : @dy_ctx (@link BT AT)) x =
+      match addr_x C x with
+      | Some addr => Some (AF addr)
+      | None => None
+      end.
+Proof.
+  induction C; simpl; eauto;
+  intros;
+  repeat des_goal; repeat des_hyp;
+  try rewrite eqb_ID_eq in *; clarify;
+  repeat rw; eauto.
+Qed.
+
+Lemma lift_ctx_M {BT AT} :
+  forall (C : dy_ctx AT) M,
+    ctx_M (lift_ctx_af C : dy_ctx (link BT AT)) M =
+      match ctx_M C M with
+      | Some CM => Some (lift_ctx_af CM)
+      | None => None
+      end.
+Proof.
+  induction C; simpl; eauto;
+  intros;
+  repeat des_goal; repeat des_hyp;
+  try rewrite eqb_ID_eq in *; clarify;
+  repeat rw; eauto.
+Qed.
+
+Definition inject_cf `{Eq BT} `{Eq AT} (Cout : dy_ctx BT) (bmem : memory BT) (cf : config AT) :=
+  match cf with
+  | Cf e C m t =>
+    Cf e ((lift_ctx_af C)[|(lift_ctx_bf Cout)|])
+      (link_mem bmem Cout m) (AF t)
+  | Rs V m t =>
+    let m := link_mem bmem Cout m in
+    let t := AF t in
+    match V with
+    | EVal (Fun x e C) =>
+      Rs (EVal (Fun x e ((lift_ctx_af C)[|(lift_ctx_bf Cout)|]))) m t
+    | EVal (Func M s e C) =>
+      Rs (EVal (Func M s e ((lift_ctx_af C)[|(lift_ctx_bf Cout)|]))) m t  
+    | MVal C =>
+      Rs (MVal ((lift_ctx_af C)[|(lift_ctx_bf Cout)|])) m t
+    end
+  end.
 
 (* projection *)
 
-Fixpoint project {T} (d : @dy_ctx T) (s : st_ctx) :=
+Fixpoint project {T} (d : dy_ctx T) (s : st_ctx) :=
   match s with
   | [[||]] => Some ([||])
   | st_binde x C =>
@@ -464,19 +1420,20 @@ Fixpoint project {T} (d : @dy_ctx T) (s : st_ctx) :=
 
 Lemma plugin_project_eq {T} {ET : Eq T} 
   (Cout Cin p : @dy_ctx T) (s : st_ctx)
-  (PROJECT : project Cin s = Some p) : project (Cout[|Cin|]) s = Some p.
+  (PROJECT : project Cin s = Some p) :
+  project (Cin[|Cout|]) s = Some p.
 Proof.
   revert Cout Cin p PROJECT.
   induction s; simpl; eauto.
   - intros.
     destruct (addr_x Cin x) eqn:ACCESS; try (inversion PROJECT; fail).
-    pose proof (plugin_ctx_addr_x x Cout Cin) as ADDR.
+    pose proof (inject_addr_x x Cout Cin) as ADDR.
     rewrite ACCESS in ADDR. rewrite ADDR.
     destruct (project Cin s) eqn:PROJ; try (inversion PROJECT; fail).
     erewrite IHs; eauto.
   - intros.
     destruct (ctx_M Cin M) eqn:ACCESS; try (inversion PROJECT; fail).
-    pose proof (plugin_ctx_ctx_M M Cout Cin) as CTX.
+    pose proof (inject_ctx_M M Cout Cin) as CTX.
     rewrite ACCESS in CTX. rewrite CTX.
     destruct (project d s1) eqn:PROJ1; try (inversion PROJECT; fail).
     destruct (project Cin s2) eqn:PROJ2; try (inversion PROJECT; fail).
@@ -488,91 +1445,6 @@ Lemma project_st_eq {T} {ET : Eq T}
   (PROJECT : project d s = Some ds) : dy_to_st ds = s.
 Proof.
   revert d ds PROJECT.
-  induction s; intros; simpl in *.
-  - inversion PROJECT; subst; eauto.
-  - destruct (addr_x d x); inversion PROJECT.
-    destruct (project d s) eqn:PROJ; inversion PROJECT.
-    specialize (IHs d d0 PROJ).
-    simpl in *. rewrite IHs. eauto.
-  - destruct (ctx_M d M); inversion PROJECT.
-    destruct (project d0 s1) eqn:PROJ1; inversion PROJECT.
-    specialize (IHs1 d0 d1 PROJ1).
-    destruct (project d s2) eqn:PROJ2; inversion PROJECT.
-    specialize (IHs2 d d2 PROJ2).
-    simpl. rewrite IHs1. rewrite IHs2. eauto.
+  induction s; ii; ss; repeat des_hyp; clarify;
+  s; f_equal; eauto.
 Qed.
-
-(* injection, deletion *)
-
-Fixpoint delete {T} `{Eq T} (Cout : @dy_ctx T) (Cin : @dy_ctx T) :=
-  match Cout, Cin with
-  | [||], Cin => Cin
-  | dy_binde x t Cout', dy_binde x' t' Cin' =>
-    if eq_eid x x' && eqb t t' then
-      delete Cout' Cin'
-    else Cin
-  | dy_bindm M Cout' Cout'', dy_bindm M' Cin' Cin'' =>
-    if eq_mid M M' && eq_ctx Cout' Cin' then
-      delete Cout'' Cin''
-    else Cin
-  | _, _ => Cin
-  end.
-
-Ltac intro_refl :=
-  assert (forall x, eq_eid x x = true) as eid_refl; [intros; apply eq_eid_eq; eauto|idtac];
-  assert (forall M, eq_mid M M = true) as mid_refl; [intros; apply eq_mid_eq; eauto|idtac];
-  assert (forall {T} `{Eq T} t, eqb t t = true) as t_refl; [intros; apply eqb_eq; eauto|idtac];
-  assert (forall {T} `{Eq T} C, eq_ctx C C = true) as ctx_refl; [intros; apply eq_ctx_eq; eauto|idtac].
-
-Lemma delete_eq :
-  forall {T} `{Eq T} (Cout Cin : dy_ctx),
-    delete Cout (Cout[|Cin|]) = Cin.
-Proof.
-  intro_refl. intros. rename H into ET. revert Cin.
-  induction Cout; simpl; eauto;    
-    try rewrite eid_refl; try rewrite mid_refl; try rewrite t_refl; try rewrite ctx_refl;
-    simpl; eauto.
-Qed.
-
-Definition plugin_ctx_v {T} `{Eq T} (Cout : @dy_ctx T) (v : @expr_value T) :=
-  match v with
-  | Fun x e C => Fun x e (Cout[|C|])
-  | Func M e s C => Func M e s (Cout[|C|])
-  end.
-
-Definition delete_ctx_v {T} `{Eq T} (Cout : @dy_ctx T) (v : @expr_value T) :=
-  match v with
-  | Fun x e C => Fun x e (delete Cout C)
-  | Func M e s C => Func M e s (delete Cout C)
-  end.
-
-(* Typeclass for concrete times *)
-Class OrderT (T : Type) `{Eq T} : Type :=
-{
-  leb : T -> T -> bool;
-  leb_refl : forall t, leb t t = true;
-  leb_trans : forall t t' t'' (LE : leb t t' = true) (LE' : leb t' t'' = true), leb t t'' = true;
-  leb_sym : forall t t' (LE : leb t t' = true) (LE' : leb t' t = true), t = t'
-}.
-
-Definition lt {T} `{OrderT T} (t1 t2 : T) :=
-  leb t1 t2 = true /\ eqb t1 t2 = false.
-
-Notation "t1 '<' t2" := (lt t1 t2).
-
-Ltac contradict :=
-  let contra := fresh "contra" in
-  assert False as contra; eauto 3; inversion contra.
-
-Lemma __R__ : forall b, b = false <-> ~ b = true.
-Proof. 
-  intros; destruct b; unfold "<>"; split; 
-  intros; try inversion H; try inversion H0; try contradict; eauto.
-Qed.
-
-Ltac refl_bool :=
-  match goal with
-  | |- _ = false => rewrite __R__; unfold "<>"
-  | |- _ <> true => rewrite <- __R__
-  | _ => idtac
-  end.
