doc/coq/basics/Basics.v
@@ -1,0 +1,117 @@
+From Coq Require Export Bool.Bool.
+From Coq Require Export Init.Nat.
+From Coq Require Export Arith.Arith.
+From Coq Require Export Arith.EqNat.
+From Coq Require Export Lia.
+From Coq Require Export Lists.List.
+From Basics Require Export tactics.
+
+Notation "x :: y" := (cons x y)
+                     (at level 60, right associativity).
+Notation "[ ]" := nil.
+Notation "[ x ; .. ; y ]" := (cons x .. (cons y []) ..).
+Notation "x ++ y" := (app x y)
+                     (at level 60, right associativity).
+
+(* Types with decidable equality *)
+Class Eq T : Type :=
+{
+  eqb : T -> T -> bool;
+  eqb_eq : forall (t t' : T), eqb t t' = true <-> t = t';
+}.
+
+Lemma eqb_comm {T} `{Eq T} :
+  forall x x', eqb x x' = eqb x' x.
+Proof.
+  intros.
+  destruct (eqb x x') eqn:EQ; destruct (eqb x' x) eqn:EQ';
+  try reflexivity;
+  try rewrite eqb_eq in *; subst;
+  try rewrite <- EQ; try rewrite <- EQ';
+  match goal with
+  | |- true = _ => symmetry
+  | _ => idtac
+  end; rewrite eqb_eq; eauto.
+Qed.
+
+Lemma eqb_neq {T} `{Eq T} : 
+  forall x x', eqb x x' = false <-> x <> x'.
+Proof.
+  intros; split; intros contra.
+  - red; intros RR. rewrite <- eqb_eq in *.
+    rewrite RR in contra. inversion contra.
+  - destruct (eqb x x') eqn:EQ; try reflexivity.
+    exfalso. apply contra. rewrite <- eqb_eq. eauto.
+Qed.
+
+Lemma t_refl {T} `{Eq T} : forall t, eqb t t = true.
+Proof. intros; apply eqb_eq; eauto. Qed.
+
+Fixpoint Inb {T} `{Eq T} t (l : list T) :=
+  match l with
+  | [] => false
+  | hd :: tl => eqb hd t || Inb t tl
+  end.
+
+Lemma Inb_eq {T} `{Eq T} :
+  forall (l : list T) (t : T),
+    Inb t l = true <-> In t l.
+Proof.
+  induction l; intros; simpl in *;
+  split; intros EQ; try contradict.
+  - repeat des_hyp;
+    simpl in *; try (inversion EQ; fail);
+    match goal with
+    | _ => left; rewrite <- eqb_eq; eauto; fail
+    | _ => right; rewrite <- IHl; eauto; fail
+    end.
+  - destruct EQ as [EQhd | EQtl].
+    subst. rewrite t_refl. eauto.
+    rewrite <- IHl in EQtl. rewrite EQtl.
+    des_goal; eauto.
+Qed.
+
+Lemma Inb_neq {T} `{Eq T} :
+  forall (l : list T) (t : T),
+    Inb t l = false <-> ~ (In t l).
+Proof.
+  induction l; intros; simpl in *;
+  split; intros NEQ; eauto.
+  - red; intros EQ.
+    destruct (eqb a t) eqn:NEQhd;
+    destruct (Inb t l) eqn:NEQtl;
+    try (inversion NEQ; fail).
+    rewrite eqb_neq in NEQhd.
+    rewrite IHl in NEQtl.
+    destruct EQ as [EQhd | EQtl];
+    match goal with
+    | _ => apply NEQhd; eauto; fail
+    | _ => apply NEQtl; eauto; fail
+    end.
+  - destruct (eqb a t) eqn:NEQhd;
+    destruct (Inb t l) eqn:NEQtl; simpl;
+    match goal with
+    | _ => reflexivity; fail
+    | [H : eqb _ _ = true |- _] =>
+      rewrite eqb_eq in H
+    | [H : Inb _ _ = true |- _] =>
+      rewrite Inb_eq in H
+    end;
+    exfalso; apply NEQ; eauto.
+Qed.
+
+(* Total order *)
+Class TotalOrder (T : Type) `{Eq T} : Type :=
+{
+  leb : T -> T -> bool;
+  leb_refl : forall t, leb t t = true;
+  leb_trans : forall t t' t'' (LE : leb t t' = true) (LE' : leb t' t'' = true), leb t t'' = true;
+  leb_sym : forall t t' (LE : leb t t' = true) (LE' : leb t' t = true), t = t';
+  leb_or : forall t t', leb t t' || leb t' t = true
+}.
+
+Definition lt {T} `{TotalOrder T} (t1 t2 : T) :=
+  leb t1 t2 = true /\ eqb t1 t2 = false.
+
+Notation "t1 '<<' t2" := (lt t1 t2) (at level 71).
+
